Adapted ADT verifications (2 holes remain relating to (non)sharing of names/structs), polishing NK en route a bit

sha/verif_hmacADT_init_part2.v
@@ -8,13 +8,16 @@ Require Import sha.spec_sha.
 Require Import sha.sha_lemmas.
 Require Import sha.HMAC_functional_prog.
 Require Import sha.HMAC256_functional_prog.
-Require Import sha.spec_hmac.
+Require Import sha.spec_hmacADT.
 Require Import vst_lemmas.
 Require Import hmac_pure_lemmas.
 Require Import hmac_common_lemmas.
 
-Require Import sha.hmac091c.
-Require Import sha.verif_hmac_init_part1.
+Require Import sha.hmac_NK.
+Require Import sha.verif_hmacADT_init_part1_5.
+(*
+Require Import sha.verif_hmacADT_init_part1.
+*)
 
 Lemma isbyte_zeroExt8: forall x, isbyteZ x -> Int.repr x = (Int.zero_ext 8 (Int.repr x)).
 Proof. intros. rewrite zero_ext_inrange. trivial.
@@ -67,38 +70,23 @@ is_int I8 Unsigned
 Proof. intros. apply Znth_map_Vint_is_int_I8.
   apply isbyte_map_ByteUnsigned.
   rewrite Zlength_map; trivial.
-Qed.
-
-Definition FIRSTN {A} i (l:list A) := firstn (Z.to_nat i) l.
-
-Lemma FIRSTN_precise {A} n (l:list A) (H: Zlength l = n): FIRSTN n l = l.
-Proof. unfold FIRSTN.
-       apply firstn_precise. subst n. apply Zlength_length; trivial. apply Zlength_nonneg.
-Qed.
-
-Lemma FIRSTN_zero {A} (l:list A): FIRSTN 0 l = []. Proof. reflexivity. Qed.
-
-Definition SKIPN {A} i (l:list A) := skipn (Z.to_nat i) l.
-
-Lemma SKIPn_short {A : Type} n (al : list A): (Zlength al <= n) -> SKIPN n al = [].
-Proof. unfold SKIPN. intros. apply skipn_short. 
-       rewrite Zlength_correct in H. rewrite <- (Nat2Z.id (length al)). 
-       rewrite (Z2Nat.inj_le _ n) in H. omega. specialize (Zlength_nonneg al); rewrite Zlength_correct. trivial.
-       specialize (Zlength_nonneg al); rewrite Zlength_correct. intros; omega. 
-Qed.
+Qed. 
 
 Lemma UPD_IPAD: forall
   (key : list Z)
-  (ZLI : Zlength
-        ( HMAC_SHA256.mkArgZ (map Byte.repr (HMAC_SHA256.mkKey key)) Ipad) =
-      64)
+(*  (ZLI : length
+        (HMAC_SHA256.mkArgZ (map Byte.repr (HMAC_SHA256.mkKey key)) Ipad) =
+      Z.to_nat 64)*)
+  (ZLI' : length
+        (HMAC_SHA256.mkArgZ (map Byte.repr (HMAC_SHA256.mkKey key)) Ipad) =
+      Z.to_nat 64)
   (i : Z)
   (I : 0 <= i < 64)
   (isbyteZQb : isbyteZ (nth (Z.to_nat i) (HMAC_SHA256.mkKey key) 0))
   (X : Znth i (map Vint (map Int.repr (HMAC_SHA256.mkKey key))) Vundef =
       Vint (Int.repr (nth (Z.to_nat i) (HMAC_SHA256.mkKey key) 0))),
 upd_reptype_array tuchar i
-  (FIRSTN i
+  (firstn (Z.to_nat i)
      (map Vint
         (map Int.repr
            (map Byte.unsigned
@@ -107,15 +95,15 @@ upd_reptype_array tuchar i
      (sem_cast_i2i I8 Unsigned
         (Vint
            (Int.repr (Z.lxor (nth (Z.to_nat i) (HMAC_SHA256.mkKey key) 0) 54))))) =
-FIRSTN (i + 1)
+firstn (Z.to_nat (i + 1))
   (map Vint
      (map Int.repr
         (map Byte.unsigned
            (HMAC_SHA256.mkArg (map Byte.repr (HMAC_SHA256.mkKey key)) Ipad)))).
 Proof. intros.
-           assert (ZLI': length (HMAC_SHA256.mkArgZ (map Byte.repr (HMAC_SHA256.mkKey key)) Ipad) = Z.to_nat 64).
-              rewrite Zlength_correct in ZLI. rewrite <- ZLI. rewrite Nat2Z.id; trivial.
-           unfold FIRSTN. unfold upd_reptype_array.
+(*           assert (ZLI': length (HMAC_SHA256.mkArgZ (map Byte.repr (HMAC_SHA256.mkKey key)) Ipad) = Z.to_nat 64).
+              rewrite Zlength_correct in ZLI. rewrite <- ZLI. rewrite Nat2Z.id; trivial.*)
+           (*unfold FIRSTN.*) unfold upd_reptype_array.
            rewrite skipn_short. Focus 2. rewrite firstn_length. unfold  HMAC_SHA256.mkArgZ in ZLI'.
                                          do 2 rewrite map_length. rewrite ZLI'.
                                          rewrite Min.min_l. unfold nat_of_Z. rewrite Z2Nat.inj_add. simpl. omega. apply I. omega.
@@ -156,20 +144,22 @@ Qed.
 
 Lemma UPD_OPAD: forall
   (key : list Z)
-  (ZLI : Zlength (HMAC_SHA256.mkArgZ (map Byte.repr (HMAC_SHA256.mkKey key)) Ipad) = 64)
-  (ZLO : Zlength (HMAC_SHA256.mkArgZ (map Byte.repr (HMAC_SHA256.mkKey key)) Opad) = 64)
+(*  (ZLI : Zlength (HMAC_SHA256.mkArgZ (map Byte.repr (HMAC_SHA256.mkKey key)) Ipad) = 64)
+  (ZLO : Zlength (HMAC_SHA256.mkArgZ (map Byte.repr (HMAC_SHA256.mkKey key)) Opad) = 64)*)
+  (ZLI' : length (HMAC_SHA256.mkArgZ (map Byte.repr (HMAC_SHA256.mkKey key)) Ipad) = Z.to_nat 64)
+  (ZLO' : length (HMAC_SHA256.mkArgZ (map Byte.repr (HMAC_SHA256.mkKey key)) Opad) = Z.to_nat 64)
   (i : Z)
   (I : 0 <= i < 64)
   (isbyteZQb : isbyteZ (nth (Z.to_nat i) (HMAC_SHA256.mkKey key) 0))
   (X : Znth i (map Vint (map Int.repr (HMAC_SHA256.mkKey key))) Vundef =
        Vint (Int.repr (nth (Z.to_nat i) (HMAC_SHA256.mkKey key) 0))),
 upd_reptype_array tuchar i
-  (FIRSTN i
+  (firstn (Z.to_nat i)
      (map Vint
         (map Int.repr
            (map Byte.unsigned
               (HMAC_SHA256.mkArg (map Byte.repr (HMAC_SHA256.mkKey key)) Opad)))) ++
-   SKIPN i
+   skipn (Z.to_nat i)
      (map Vint
         (map Int.repr
            (map Byte.unsigned
@@ -178,24 +168,24 @@ upd_reptype_array tuchar i
      (Int.zero_ext 8
         (Int.xor (Int.repr 92)
            (Int.repr (nth (Z.to_nat i) (HMAC_SHA256.mkKey key) 0))))) =
-FIRSTN (i + 1)
+firstn (Z.to_nat (i + 1))
   (map Vint
      (map Int.repr
         (map Byte.unsigned
            (HMAC_SHA256.mkArg (map Byte.repr (HMAC_SHA256.mkKey key)) Opad)))) ++
-SKIPN (i + 1)
+skipn (Z.to_nat (i + 1))
   (map Vint
      (map Int.repr
         (map Byte.unsigned
            (HMAC_SHA256.mkArg (map Byte.repr (HMAC_SHA256.mkKey key)) Ipad)))).
 Proof. intros.
-           assert (ZLI': length (HMAC_SHA256.mkArgZ (map Byte.repr (HMAC_SHA256.mkKey key)) Ipad) = Z.to_nat 64).
+          (* assert (ZLI': length (HMAC_SHA256.mkArgZ (map Byte.repr (HMAC_SHA256.mkKey key)) Ipad) = Z.to_nat 64).
                  rewrite Zlength_correct in ZLI. rewrite <- ZLI. rewrite Nat2Z.id; trivial. 
            assert (ZLO': length (HMAC_SHA256.mkArgZ (map Byte.repr (HMAC_SHA256.mkKey key)) Opad) = Z.to_nat 64).
-              rewrite Zlength_correct in ZLO. rewrite <- ZLO. rewrite Nat2Z.id; trivial.
-           unfold FIRSTN. unfold upd_reptype_array, nat_of_Z.
+              rewrite Zlength_correct in ZLO. rewrite <- ZLO. rewrite Nat2Z.id; trivial.*)
+           (*unfold FIRSTN.*) unfold upd_reptype_array, nat_of_Z.
            rewrite force_lengthn_long.
-           Focus 2. unfold SKIPN; rewrite app_length, firstn_length, skipn_length.
+           Focus 2. (*unfold SKIPN;*) rewrite app_length, firstn_length, skipn_length.
            unfold HMAC_SHA256.mkArgZ in ZLI', ZLO'. 
            do 2 rewrite map_length. rewrite ZLO'. 
            do 2 rewrite map_length. rewrite ZLI', Min.min_l. 2: apply Z2Nat.inj_le; omega.
@@ -245,77 +235,78 @@ Proof. intros.
               rewrite skipn_app2; rewrite firstn_length, Min.min_l.
               Focus 2. do 2 rewrite map_length. unfold HMAC_SHA256.mkArgZ in ZLO'; rewrite ZLO'.
                        apply Z2Nat.inj_le; omega.
-              rewrite minus_diag. simpl. unfold SKIPN. rewrite Z2Nat.inj_add, <- skipn_skipn. reflexivity.
-              omega. omega. omega.
+              rewrite minus_diag. simpl. (*unfold SKIPN.*) rewrite (*Z2Nat.inj_add,*) <- skipn_skipn. reflexivity.
+              omega. (*omega. omega.*)
               do 2 rewrite map_length. unfold HMAC_SHA256.mkArgZ in ZLO'; rewrite ZLO'.
                        apply Z2Nat.inj_le; omega.
 Qed.
 
-Definition postResetHMS key (iS oS: s256state): hmacstate :=
-  (emptySha, (iS, (oS, 
-   (if zlt 64 (Zlength key) then Vint (Int.repr 32) else Vint (Int.repr (Zlength key)), 
-   map Vint (map Int.repr (HMAC_SHA256.mkKey key)))))).
+Definition postResetHMS (ctxS iS oS: s256state): hmacstate :=
+  (ctxS, (iS, oS)).
 
-Definition initPostResetConditional r (c:val) (k: val) h key iS oS: mpred:=
+Definition initPostResetConditional l r (c:val) (k: val) h key ctxS iS oS: mpred:=
   match k with
     Vint z => if Int.eq z Int.zero
               then if zeq r Z0 then hmacstate_PreInitNull key h c else FF
               else FF
   | Vptr b ofs => if zeq r 0 then FF
-                  else !!(Forall isbyteZ key) &&
-                       ((data_at Tsh t_struct_hmac_ctx_st (postResetHMS key iS oS) c) *
+                  else EX ll:_, !!(Forall isbyteZ key/\ has_lengthK ll key /\ l = Vint(Int.repr ll)) &&
+                       ((data_at Tsh t_struct_hmac_ctx_st (postResetHMS ctxS iS oS) c) *
                         (data_at Tsh (tarray tuchar (Zlength key)) (map Vint (map Int.repr key)) (Vptr b ofs)))
   | _ => FF
   end.
 
 Lemma init_part2: forall
 (Espec : OracleKind)
-(c : val)
 (k : val)
-(l : Z)
+(l : val)
 (key : list Z)
 (kv : val)
 (h1 : hmacabs)
-(KL1 : l = Zlength key)
-(KL2 : 0 <= l <= Int.max_signed)
-(KL3 : l * 8 < two_p 64)
 (ctx' : name _ctx)
 (key' : name _key)
 (len' : name _len)
 (pad : val)
-(Delta := initialized _reset 
-       (func_tycontext f_HMAC_Init HmacVarSpecs HmacFunSpecs))
+(ckb : block)
+(ckoff : int)
 (cb : block)
 (cofs : int)
 (r : Z)
-(HC : c = Vptr cb cofs)
 (R : r = 0 \/ r = 1)
 (PostResetBranch : environ -> mpred)
 (HeqPostResetBranch : PostResetBranch =
-                     EX  shaStates
-                     : s256abs * (s256state * (s256abs * s256state)),
-                     PROP 
-                     (innerShaInit (map Byte.repr (HMAC_SHA256.mkKey key))
-                        (fst shaStates) /\
-                      s256_relate (fst shaStates) (fst (snd shaStates)) /\
-                      outerShaInit (map Byte.repr (HMAC_SHA256.mkKey key))
-                        (fst (snd (snd shaStates))) /\
-                      s256_relate (fst (snd (snd shaStates)))
-                        (snd (snd (snd shaStates))))
-                     LOCAL  (lvar _pad (tarray tuchar 64) pad;
-                     temp _ctx (Vptr cb cofs); temp _key k;
-                     temp _len (Vint (Int.repr l)); gvar sha._K256 kv)
-                     SEP  (`(data_at_ Tsh (tarray tuchar 64) pad);
-                     `(initPostResetConditional r c k h1 key
-                         (fst (snd shaStates)) (snd (snd (snd shaStates))));
-                     `(K_vector kv))),
-semax Delta
+                     EX  iSA : s256abs,
+                     (EX  iS : s256state,
+                      (EX  oSA : s256abs,
+                       (EX  oS : s256state,
+                        (EX  CONT : s256state,
+                         PROP 
+                         (innerShaInit
+                            (map Byte.repr (HMAC_SHA256.mkKey key)) iSA /\
+                          s256_relate iSA iS /\
+                          outerShaInit
+                            (map Byte.repr (HMAC_SHA256.mkKey key)) oSA /\
+                          s256_relate oSA oS)
+                         LOCAL  (lvar _pad (tarray tuchar 64) pad;
+                         lvar _ctx_key (tarray tuchar 64) (Vptr ckb ckoff);
+                         temp _ctx (Vptr cb cofs); temp _key k; temp _len l;
+                         gvar sha._K256 kv)
+                         SEP  (`(data_at_ Tsh (tarray tuchar 64) pad);
+                         `(data_at_ Tsh (Tarray tuchar 64 noattr)
+                             (Vptr ckb ckoff));
+                         `(initPostResetConditional l r (Vptr cb cofs) k h1
+                             key CONT iS oS); `(K_vector kv))))))),
+semax
+  (initialized_list [_reset]
+     (func_tycontext f_HMAC_Init HmacVarSpecs HmacFunSpecs))
   (PROP  ()
-   LOCAL  (temp _reset (Vint (Int.repr r)); lvar _pad (tarray tuchar 64) pad;
-   temp _ctx (Vptr cb cofs); temp _key k; temp _len (Vint (Int.repr l));
-   gvar sha._K256 kv)
+   LOCAL  (temp _reset (Vint (Int.repr r));
+   lvar _ctx_key (tarray tuchar 64) (Vptr ckb ckoff);
+   lvar _pad (tarray tuchar 64) pad; temp _ctx (Vptr cb cofs); temp _key k;
+   temp _len l; gvar sha._K256 kv)
    SEP  (`(data_at_ Tsh (tarray tuchar 64) pad);
-   `(initPostKeyNullConditional r (Vptr cb cofs) k h1 key); `(K_vector kv)))
+   `(initPostKeyNullConditional l r (Vptr cb cofs) k h1 key (Vptr ckb ckoff));
+   `(K_vector kv)))
   (Sifthenelse (Etempvar _reset tint)
      (Ssequence
         (Sfor (Sset _i (Econst_int (Int.repr 0) tint))
@@ -325,11 +316,7 @@ semax Delta
               (Sset _aux
                  (Ecast
                     (Ederef
-                       (Ebinop Oadd
-                          (Efield
-                             (Ederef
-                                (Etempvar _ctx (tptr t_struct_hmac_ctx_st))
-                                t_struct_hmac_ctx_st) _key (tarray tuchar 64))
+                       (Ebinop Oadd (Evar _ctx_key (tarray tuchar 64))
                           (Etempvar _i tint) (tptr tuchar)) tuchar) tuchar))
               (Ssequence
                  (Sset _aux
@@ -377,13 +364,9 @@ semax Delta
                           (Ecast
                              (Ederef
                                 (Ebinop Oadd
-                                   (Efield
-                                      (Ederef
-                                         (Etempvar _ctx
-                                            (tptr t_struct_hmac_ctx_st))
-                                         t_struct_hmac_ctx_st) _key
-                                      (tarray tuchar 64)) (Etempvar _i tint)
-                                   (tptr tuchar)) tuchar) tuchar))
+                                   (Evar _ctx_key (tarray tuchar 64))
+                                   (Etempvar _i tint) (tptr tuchar)) tuchar)
+                             tuchar))
                        (Sassign
                           (Ederef
                              (Ebinop Oadd (Evar _pad (tarray tuchar 64))
@@ -427,83 +410,94 @@ semax Delta
            (EX  h : hmacabs,
             PROP  (hmacInit key h)
             LOCAL ()
-            SEP  (`(hmacstate_ h c); `(initPostKey k key); `(K_vector kv))))
-        (stackframe_of f_HMAC_Init))).
+            SEP  (`(hmacstate_ h (Vptr cb cofs)); `(initPostKey k key);
+            `(K_vector kv)))) (stackframe_of f_HMAC_Init))).
 Proof. intros.
-forward_if PostResetBranch. 
+  forward_if PostResetBranch. 
   { (* THEN*)
     rename H into r_true. 
     remember (map Vint (map Int.repr 
               (map Byte.unsigned (HMAC_SHA256.mkArg (map Byte.repr (HMAC_SHA256.mkKey key)) Ipad)))) as IPADcont.
     remember (map Vint (map Int.repr 
               (map Byte.unsigned (HMAC_SHA256.mkArg (map Byte.repr (HMAC_SHA256.mkKey key)) Opad)))) as OPADcont.
-    assert (ZLI: Zlength (HMAC_SHA256.mkArgZ (map Byte.repr (HMAC_SHA256.mkKey key)) Ipad) = 64).
+    assert (ZLI: length (HMAC_SHA256.mkArgZ (map Byte.repr (HMAC_SHA256.mkKey key)) Ipad) = Z.to_nat 64).
+            apply Zlength_length. omega.
             rewrite Zlength_mkArgZ.
             repeat rewrite map_length. rewrite mkKey_length.
             unfold SHA256.BlockSize; simpl. trivial. 
-    assert (ZLO: Zlength (HMAC_SHA256.mkArgZ (map Byte.repr (HMAC_SHA256.mkKey key)) Opad) = 64).
+    assert (ZLO: length (HMAC_SHA256.mkArgZ (map Byte.repr (HMAC_SHA256.mkKey key)) Opad) = Z.to_nat 64).
+            apply Zlength_length. omega.
             rewrite Zlength_mkArgZ.
             repeat rewrite map_length. rewrite mkKey_length.
             unfold SHA256.BlockSize; simpl. trivial. 
     unfold data_at_, tarray.
-    assert_PROP (isptr pad). entailer!. apply isptrD in H. destruct H as [pb [pofs Hpad]]. subst pad.
-    apply semax_pre with (P':=PROP  (r<>0 /\ Forall isbyteZ key)
+    assert_PROP (isptr pad). entailer!. apply isptrD in H; destruct H as [pb [pofs Hpad]]. subst pad. 
+    unfold initPostKeyNullConditional.
+    apply semax_pre with (P':=EX ll:_, EX CONT:_,
+         PROP  (r<>0 /\ Forall isbyteZ key/\ has_lengthK ll key /\ l = Vint(Int.repr ll))
          LOCAL  (temp _reset (Vint (Int.repr r));
+           lvar _ctx_key (Tarray tuchar 64 noattr) (Vptr ckb ckoff);
            lvar _pad (Tarray tuchar 64 noattr) (Vptr pb pofs);
-           temp _ctx (Vptr cb cofs); temp _key k; temp _len (Vint (Int.repr l));
+           temp _ctx (Vptr cb cofs); temp _key k; temp _len l;
            gvar sha._K256 kv)
-         SEP  (`(K_vector kv);
-               `(data_at Tsh (Tarray tuchar 64 noattr)
-                   (default_val (Tarray tuchar 64 noattr)) (Vptr pb pofs));
-               `(data_at Tsh t_struct_hmac_ctx_st (keyedHMS key) (Vptr cb cofs));
-               `(data_at Tsh (tarray tuchar (Zlength key)) (map Vint (map Int.repr key)) k))).
+         SEP  (`(data_at Tsh t_struct_hmac_ctx_st CONT (Vptr cb cofs));
+               `(data_at Tsh (tarray tuchar 64) (map Vint (map Int.repr (HMAC_SHA256.mkKey key)))
+                      (Vptr ckb ckoff));
+               `(data_at Tsh (tarray tuchar (Zlength key)) (map Vint (map Int.repr key))
+                      k);
+              `(K_vector kv);
+              `(data_at Tsh (Tarray tuchar 64 noattr)
+                  (default_val (Tarray tuchar 64 noattr)) (Vptr pb pofs)))).
     { clear HeqPostResetBranch PostResetBranch.
-      unfold initPostKeyNullConditional. entailer. 
+      unfold initPostKeyNullConditional. entailer.
       destruct key'; try contradiction.
       (*integer, ie key==NULL*)
-          simpl in TC0. subst i. simpl. if_tac. subst r. inversion r_true. 
-          apply andp_right. entailer. entailer!.
+          simpl in TC0. subst i. simpl. if_tac. subst r. inversion r_true. normalize.
       (*key == Vptr*)
-       if_tac. subst r. inversion r_true.
-          entailer!.
-    } 
-    normalize. destruct R; subst r. omega. clear H. rename H0 into isbyte_key.
-    assert_PROP (isptr k). entailer!. apply isptrD in H; destruct H as [kb [kofs HK]]. 
-    subst k.
+       if_tac. normalize. entailer. apply (exp_right ll). 
+       apply (exp_right CONT). entailer!.
+    }
+    apply extract_exists_pre; intros ll.
+    apply extract_exists_pre; intros CONT. normalize. subst l; rename ll into l.
+    rename H0 into isbyte_key. rename H1 into KL.
+    destruct R; subst r. omega. clear H.
+    assert_PROP (isptr k). entailer!. apply isptrD in H; destruct H as [kb [kofs HK]]. subst k.
 
-    eapply semax_seq'. (*TODO: using forward_seq here introduces another Delta0 in goal2 - but 
-                          it worked fine before I split this off into file XXX_part2.v *)
+    forward_seq. 
     instantiate (1:= 
       (PROP  ()
        LOCAL  (temp _reset (Vint (Int.repr 1));
-          lvar _pad (Tarray tuchar 64 noattr) (Vptr pb pofs);
-          temp _ctx (Vptr cb cofs); temp _key (Vptr kb kofs);
-          temp _len (Vint (Int.repr l)); gvar sha._K256 kv)
-       SEP 
-        (`(K_vector kv);
+         lvar _ctx_key (Tarray tuchar 64 noattr) (Vptr ckb ckoff);
+         lvar _pad (Tarray tuchar 64 noattr) (Vptr pb pofs);
+         temp _ctx (Vptr cb cofs); temp _key (Vptr kb kofs);
+         temp _len (Vint (Int.repr l)); gvar sha._K256 kv)
+       SEP  (`(K_vector kv);
          `(data_at Tsh (Tarray tuchar 64 noattr) IPADcont (Vptr pb pofs));
-         `(data_at Tsh t_struct_hmac_ctx_st (keyedHMS key) (Vptr cb cofs));
-         `(data_at Tsh (tarray tuchar (Zlength key)) (map Vint (map Int.repr key)) (Vptr kb kofs))))).
-
+         `(data_at Tsh t_struct_hmac_ctx_st CONT (Vptr cb cofs));
+         `(data_at Tsh (tarray tuchar 64)
+             (map Vint (map Int.repr (HMAC_SHA256.mkKey key))) (Vptr ckb ckoff));
+         `(data_at Tsh (tarray tuchar (Zlength key)) (map Vint (map Int.repr key))
+             (Vptr kb kofs))))).
     { (*ipad loop*)
       forward_for_simple_bound' 64 (EX i:Z, 
         (PROP  ()
          LOCAL  (temp _reset (Vint (Int.repr 1));
-          lvar _pad (Tarray tuchar 64 noattr) (Vptr pb pofs);
-          temp _ctx (Vptr cb cofs); temp _key (Vptr kb kofs);
-          temp _len (Vint (Int.repr l)); gvar sha._K256 kv)
+           lvar _ctx_key (Tarray tuchar 64 noattr) (Vptr ckb ckoff);
+           lvar _pad (Tarray tuchar 64 noattr) (Vptr pb pofs);
+           temp _ctx (Vptr cb cofs); temp _key (Vptr kb kofs);
+           temp _len (Vint (Int.repr l)); gvar sha._K256 kv)
          SEP  (`(K_vector kv);
-               `(data_at Tsh (Tarray tuchar 64 noattr)
-                   (FIRSTN i IPADcont) (Vptr pb pofs));
-               `(data_at Tsh t_struct_hmac_ctx_st (keyedHMS key) (Vptr cb cofs));
-               `(data_at Tsh (tarray tuchar (Zlength key)) (map Vint (map Int.repr key))
-                  (Vptr kb kofs))))).
-      { (*precondition implies "invariant"*) 
+          `(data_at Tsh (Tarray tuchar 64 noattr) (firstn (Z.to_nat i) IPADcont) (Vptr pb pofs));
+          `(data_at Tsh t_struct_hmac_ctx_st CONT (Vptr cb cofs));
+          `(data_at Tsh (tarray tuchar 64)
+              (map Vint (map Int.repr (HMAC_SHA256.mkKey key))) (Vptr ckb ckoff));
+         `(data_at Tsh (tarray tuchar (Zlength key)) (map Vint (map Int.repr key))
+              (Vptr kb kofs))))).
+      { (*precondition implies "invariant"*)
         clear HeqPostResetBranch. entailer!. 
-      }
-      { unfold normal_ret_assert. simpl. intros rho. entailer!. cancel.
-        rewrite FIRSTN_precise. cancel.
-         do 2 rewrite Zlength_map. apply ZLI. 
+      } 
+      { unfold normal_ret_assert. rewrite firstn_precise. simpl. intros rho. entailer!.
+        subst IPADcont; clear - ZLI. do 2 rewrite map_length. apply ZLI.
       }
       { rename H into I. 
         subst PostResetBranch.
@@ -521,14 +515,14 @@ forward_if PostResetBranch.
               Focus 2. repeat rewrite map_length. rewrite mkKey_length. unfold SHA256.BlockSize; simpl. apply (Z2Nat.inj_lt _ 64); omega. 
             repeat rewrite map_nth. rewrite Qb. trivial. 
           }
-        forward. entailer!. 
+        forward. entailer!.
         (*apply prop_right.*) rewrite X. simpl. rewrite <- isbyte_zeroExt8'; trivial.
                apply (isbyteZ_range _ isbyteZQb). 
         unfold force_val. rewrite sem_cast_i2i_correct_range.
             Focus 2. apply Znth_map_Vint_is_int_I8.
                      apply isbyteZ_mkKey. assumption.
                      rewrite Zlength_correct, mkKey_length. unfold SHA256.BlockSize; simpl; assumption.
-        rewrite X. 
+        rewrite X.
         forward v. subst v.
         unfold Int.xor. 
         rewrite Int.unsigned_repr. 2: rewrite int_max_unsigned_eq; omega.
@@ -539,51 +533,61 @@ forward_if PostResetBranch.
         rewrite Z.lxor_comm. remember (Vint (Int.repr (Z.lxor qb 54))) as xorval.
         forward. simpl. intros rho. entailer. cancel.
         rewrite Z.lxor_comm in isbyteXOR.
-        rewrite UPD_IPAD; try assumption. cancel. 
+        rewrite UPD_IPAD; try assumption. cancel.
       }
     }
 
     (*continuation after ipad-loop*)   
     unfold_data_at 2%nat. normalize.
-    rewrite (field_at_data_at Tsh t_struct_hmac_ctx_st [StructField _i_ctx]); try reflexivity. normalize.
+    rewrite (field_at_data_at Tsh t_struct_hmac_ctx_st [StructField _i_ctx]). 
     (*extract field-address info before doing anything else*)
        assert_PROP (isptr (field_address t_struct_hmac_ctx_st [StructField _i_ctx]
           (Vptr cb cofs))). entailer!.
-       apply isptrD in H. destruct H as [? [? PT]]; rewrite PT.
-       unfold field_address in PT.
-       destruct(field_compatible_dec t_struct_hmac_ctx_st [StructField _i_ctx]
-           (Vptr cb cofs)); simpl in PT; inversion PT; clear PT.
-       subst x x0. 
-       unfold nested_field_offset2; simpl. 
+       apply isptrD in H. destruct H as [cbI [cIoff COffI]]. rewrite COffI in *.
+    unfold field_address in COffI.
+    remember (field_compatible_dec t_struct_hmac_ctx_st [StructField _i_ctx]
+              (Vptr cb cofs)) as s.
+    destruct s; simpl in *; inversion COffI. simpl in *. subst cbI. rewrite COffI. clear COffI. 
 
     (*Call to _SHA256_Init*)
-    forward_call' (Vptr cb (Int.add cofs (Int.repr 108))).
+    forward_call' (Vptr cb cIoff).
+    { (*rewrite <- H1 in *; clear H1. entailer. cIoff.*)
+       assert (FR: Frame = [
+          (field_at Tsh t_struct_hmac_ctx_st [StructField _o_ctx] (snd (snd CONT)) (Vptr cb cofs));
+          (field_at Tsh t_struct_hmac_ctx_st [StructField _md_ctx] (fst CONT) (Vptr cb cofs));
+          (K_vector kv); (data_at Tsh (Tarray tuchar 64 noattr) IPADcont (Vptr pb pofs));
+          (data_at Tsh (tarray tuchar 64)
+             (map Vint (map Int.repr (HMAC_SHA256.mkKey key))) (Vptr ckb ckoff));
+          (data_at Tsh (tarray tuchar (Zlength key)) (map Vint (map Int.repr key))
+             (Vptr kb kofs))]).
+        subst Frame; reflexivity.
+      rewrite FR; clear FR Frame. 
+      entailer. cancel.
+      assert (TP: nested_field_type2 t_struct_hmac_ctx_st [StructField _i_ctx]
+                  = sha.t_struct_SHA256state_st).
+        admit. (*TODO: struct equality
+        unfold nested_field_type2. simpl. unfold sha.t_struct_SHA256state_st. 
+        f_equal. reflexivity. unfold  sha.t_struct_SHA256state_st.*)
+      erewrite data_at_type_changable. 2: eassumption. 2: apply JMeq.JMeq_refl. cancel.
+    }
 
     (*Call to _SHA256_Update*)
-    Opaque firstn. 
+    Opaque firstn.
     forward_call' (init_s256abs, 
             HMAC_SHA256.mkArgZ (map Byte.repr (HMAC_SHA256.mkKey key)) Ipad,
-            Vptr cb (Int.add cofs (Int.repr 108)),
-            Vptr pb pofs, Tsh, 64, kv) ipadSHAabs.
-      { assert (FR: Frame = [
-           field_at Tsh t_struct_hmac_ctx_st [StructField _key_length]
-              (if zlt 64 (Zlength key)
-               then Vint (Int.repr 32)
-               else Vint (Int.repr (Zlength key))) (Vptr cb cofs);
-           field_at Tsh t_struct_hmac_ctx_st [StructField _key]
-              (map Vint (map Int.repr (HMAC_SHA256.mkKey key))) (Vptr cb cofs);
-           field_at Tsh t_struct_hmac_ctx_st [StructField _o_ctx] emptySha
-              (Vptr cb cofs);
-           field_at Tsh t_struct_hmac_ctx_st [StructField _md_ctx] emptySha
-              (Vptr cb cofs);
-           data_at Tsh (tarray tuchar (Zlength key)) (map Vint (map Int.repr key))
-              (Vptr kb kofs)]).
-          subst Frame; reflexivity.
-        rewrite FR; clear FR Frame. 
-        unfold data_block, tarray. rewrite ZLI. simpl. normalize.
-        apply andp_right. apply prop_right. apply isbyte_map_ByteUnsigned.
-        subst IPADcont. cancel. 
-      }
+            Vptr cb cIoff, Vptr pb pofs, Tsh, 64, kv) ipadSHAabs.
+    { assert (FR: Frame = [
+        (field_at Tsh t_struct_hmac_ctx_st [StructField _o_ctx] emptySha (Vptr cb cofs));
+        (field_at Tsh t_struct_hmac_ctx_st [StructField _md_ctx] emptySha (Vptr cb cofs));
+        (data_at Tsh (tarray tuchar 64) (map Vint (map Int.repr (HMAC_SHA256.mkKey key))) (Vptr ckb ckoff));
+        data_at Tsh (tarray tuchar (Zlength key)) (map Vint (map Int.repr key)) (Vptr kb kofs) ]).
+        subst Frame; reflexivity.
+      rewrite FR; clear FR Frame. 
+      entailer!.
+      unfold data_block. rewrite Zlength_correct. rewrite ZLI. entailer!. 
+      apply andp_right. 
+        simpl. apply prop_right. apply isbyte_map_ByteUnsigned. cancel. 
+    }
       { clear Frame HeqPostResetBranch HeqOPADcont; subst IPADcont.
         rewrite Zlength_mkArgZ. repeat rewrite map_length. rewrite mkKey_length. 
         unfold SHA256.BlockSize; simpl. rewrite int_max_unsigned_eq.
@@ -597,65 +601,56 @@ forward_if PostResetBranch.
             repeat rewrite map_length. rewrite mkKey_length. simpl. omega. 
     Transparent firstn. 
 
-    (*essentially the same for opad*) 
-    eapply semax_seq'. (* TODO: using forward_seq here introduces another Delta0 in goal2 - but 
-                          it worked fine before I split this off into file XXX_part2.v *)
-
-    instantiate (1:=  (PROP  ()
-      LOCAL  (temp _reset (Vint (Int.repr 1));
-           lvar _pad (Tarray tuchar 64 noattr) (Vptr pb pofs);
-           temp _ctx (Vptr cb cofs); temp _key (Vptr kb kofs);
-           temp _len (Vint (Int.repr l)); gvar sha._K256 kv)
-      SEP  (`(K_vector kv);
-         `(sha256state_ ipadSHAabs (Vptr cb (Int.add cofs (Int.repr 108))));
-         `(field_at Tsh t_struct_hmac_ctx_st [StructField _key_length]
-             (if zlt 64 (Zlength key)
-              then Vint (Int.repr 32)
-              else Vint (Int.repr (Zlength key))) (Vptr cb cofs));
-         `(field_at Tsh t_struct_hmac_ctx_st [StructField _key]
-             (map Vint (map Int.repr (HMAC_SHA256.mkKey key))) (Vptr cb cofs));
-   
+    (*essentially the same for opad*)
+    forward_seq.
+    instantiate (1:= 
+  (PROP  ()
+   LOCAL  (temp _reset (Vint (Int.repr 1));
+      lvar _ctx_key (Tarray tuchar 64 noattr) (Vptr ckb ckoff);
+      lvar _pad (Tarray tuchar 64 noattr) (Vptr pb pofs);
+      temp _ctx (Vptr cb cofs); temp _key (Vptr kb kofs);
+      temp _len (Vint (Int.repr l)); gvar sha._K256 kv)
+        SEP  (`(K_vector kv);
+         `(sha256state_ ipadSHAabs (Vptr cb cIoff));
          `(data_at Tsh (Tarray tuchar 64 noattr) OPADcont (Vptr pb pofs));
-
          `(field_at Tsh t_struct_hmac_ctx_st [StructField _o_ctx] emptySha (Vptr cb cofs));
-
          `(field_at Tsh t_struct_hmac_ctx_st [StructField _md_ctx] emptySha (Vptr cb cofs));
+         `(data_at Tsh (tarray tuchar 64)
+            (map Vint (map Int.repr (HMAC_SHA256.mkKey key))) (Vptr ckb ckoff));
          `(data_at Tsh (tarray tuchar (Zlength key)) (map Vint (map Int.repr key))
-             (Vptr kb kofs))))).
-
-    { (*opad loop*)
+            (Vptr kb kofs))))).
+    { (*opad loop*) 
+     Opaque firstn. Opaque skipn.
       forward_for_simple_bound' 64 (EX i:Z, 
-       (PROP  ()
-        LOCAL  (temp _reset (Vint (Int.repr 1));
+        (PROP  ()
+         LOCAL  (temp _reset (Vint (Int.repr 1));
+            lvar _ctx_key (Tarray tuchar 64 noattr) (Vptr ckb ckoff);
             lvar _pad (Tarray tuchar 64 noattr) (Vptr pb pofs);
             temp _ctx (Vptr cb cofs); temp _key (Vptr kb kofs);
             temp _len (Vint (Int.repr l)); gvar sha._K256 kv)
-        SEP  (`(K_vector kv);
-         `(sha256state_ ipadSHAabs (Vptr cb (Int.add cofs (Int.repr 108))));
-         `(data_at Tsh (Tarray tuchar 64 noattr) ((FIRSTN i OPADcont)++(SKIPN i IPADcont)) (Vptr pb pofs));
+         SEP  (`(K_vector kv);
+           `(sha256state_ ipadSHAabs (Vptr cb (Int.add cofs (Int.repr 108))));
   
-         `(field_at Tsh t_struct_hmac_ctx_st [StructField _key_length]
-            (if zlt 64 (Zlength key)
-             then Vint (Int.repr 32)
-             else Vint (Int.repr (Zlength key))) (Vptr cb cofs));
-        `(field_at Tsh t_struct_hmac_ctx_st [StructField _key]
-           (map Vint (map Int.repr (HMAC_SHA256.mkKey key))) (Vptr cb cofs));
-         `(field_at Tsh t_struct_hmac_ctx_st [StructField _o_ctx] emptySha (Vptr cb cofs));
-        `(field_at Tsh t_struct_hmac_ctx_st [StructField _md_ctx] emptySha (Vptr cb cofs));
-        `(data_at Tsh (tarray tuchar (Zlength key)) (map Vint (map Int.repr key)) (Vptr kb kofs))))).
+           `(data_at Tsh (Tarray tuchar 64 noattr) ((firstn (Z.to_nat i) OPADcont)++(skipn (Z.to_nat i) IPADcont)) (Vptr pb pofs));
+           `(data_at Tsh (tarray tuchar 64)
+              (map Vint (map Int.repr (HMAC_SHA256.mkKey key))) (Vptr ckb ckoff));
+           `(field_at Tsh t_struct_hmac_ctx_st [StructField _o_ctx] emptySha (Vptr cb cofs));
+           `(field_at Tsh t_struct_hmac_ctx_st [StructField _md_ctx] emptySha (Vptr cb cofs));
+          `(data_at Tsh (tarray tuchar (Zlength key)) (map Vint (map Int.repr key)) (Vptr kb kofs))))).
       { (*precondition implies "invariant"*)
         clear HeqPostResetBranch.
         unfold data_block. entailer!. cancel. 
-        unfold SKIPN; simpl. rewrite ZLI; cancel.            
+       (* unfold SKIPN;*) simpl. rewrite Zlength_correct, ZLI; cancel.            
       }
       { unfold normal_ret_assert. simpl. intros rho. entailer!. cancel.
-        rewrite FIRSTN_precise.
-         rewrite SKIPn_short. rewrite app_nil_r.
+        rewrite firstn_precise.
+         rewrite skipn_short. rewrite app_nil_r.
          cancel.
-         do 2 rewrite Zlength_map. unfold HMAC_SHA256.mkArgZ in ZLI; rewrite ZLI. omega. 
-         do 2 rewrite Zlength_map. unfold HMAC_SHA256.mkArgZ in ZLO; rewrite ZLO; trivial. 
+         do 2 rewrite map_length. unfold HMAC_SHA256.mkArgZ in ZLI; rewrite ZLI. omega. 
+         do 2 rewrite map_length. unfold HMAC_SHA256.mkArgZ in ZLO; rewrite ZLO; trivial. 
       }
-      { rename H into I. 
+      { (*unfold_data_at 1%nat. normalize.*)
+        rename H into I.
         assert (Xb: exists qb, nth (Z.to_nat i) (HMAC_SHA256.mkKey key) Z0 = qb /\ isbyteZ qb).
           { destruct (nth_mapIn (Z.to_nat i) (HMAC_SHA256.mkKey key) 0) as [? [? ?]].
              rewrite mkKey_length.
@@ -671,79 +666,48 @@ forward_if PostResetBranch.
             repeat rewrite map_nth. rewrite Qb. trivial. 
           }
         forward.
-        { entailer!. 
-          (*apply prop_right.*) rewrite X. simpl. rewrite <- isbyte_zeroExt8'; trivial.
-                apply (isbyteZ_range _ isbyteZQb). 
+        { entailer!. Transparent firstn. simpl. rewrite X. simpl. rewrite <- isbyte_zeroExt8'; trivial.
+                apply (isbyteZ_range _ isbyteZQb).
         }
-        unfold force_val. rewrite sem_cast_i2i_correct_range.
+        Transparent firstn. Transparent skipn. simpl. unfold force_val. rewrite sem_cast_i2i_correct_range.
         Focus 2. apply Znth_map_Vint_is_int_I8.
                      apply isbyteZ_mkKey. assumption.
                      rewrite Zlength_correct, mkKey_length. unfold SHA256.BlockSize; simpl; assumption.
         rewrite X.
         forward.
-        entailer!. cancel. 
+        entailer!.
         rewrite UPD_OPAD; try assumption. cancel.
       }
     }
-    (*continuation after opad-loop*)  
+
+    (*continuation after opad-loop*)
     rewrite (field_at_data_at Tsh t_struct_hmac_ctx_st [StructField _o_ctx]).
-    rewrite (field_at_data_at Tsh t_struct_hmac_ctx_st [StructField _key]).
-    assert_PROP (isptr (field_address t_struct_hmac_ctx_st [StructField _key] (Vptr cb cofs)) /\  
-                 isptr (field_address t_struct_hmac_ctx_st [StructField _o_ctx] (Vptr cb cofs))).
+    assert_PROP (isptr (field_address t_struct_hmac_ctx_st [StructField _o_ctx] (Vptr cb cofs))).
     { entailer!. }
-    destruct H as [HKEY HOPAD]. 
-    apply isptrD in HOPAD. destruct HOPAD as [cbO [cOoff COffO]]. rewrite COffO in *.
+    apply isptrD in H; destruct H as [cbO [cOoff COffO]]. rewrite COffO in *.
     unfold field_address in COffO.
     remember (field_compatible_dec t_struct_hmac_ctx_st [StructField _o_ctx]
               (Vptr cb cofs)) as s.
-    destruct s; simpl in *; inversion COffO. simpl in *. subst cbO cOoff. 
-    apply isptrD in HKEY. destruct HKEY as [cbK [cKoff COffK]]. rewrite COffK in *.
-    unfold field_address in COffK.
-    remember (field_compatible_dec t_struct_hmac_ctx_st [StructField _key]
-              (Vptr cb cofs)) as s.
-    destruct s; simpl in *; inversion COffK. simpl in *. subst cbK cKoff.
-
-    (*Call to _SHA256_Init*) 
-    (*TODO: one of the most recent changes in floyd (or elsewhere?) meant
-    that I have to do the following unfold here t get forward_call' to apply*)
+    destruct s; simpl in *; inversion COffO; clear COffO. simpl in *. subst cbO cOoff.
+   
+    (*Call to _SHA256_Init*)  
     forward_call' (Vptr cb (Int.add cofs (Int.repr 216))).
-
+    
     (* Call to sha_update*)
-    (*TODO: the old proof started like this:
-      forward_call (init_s256abs, 
+    Opaque firstn.  
+    forward_call' (init_s256abs, 
             HMAC_SHA256.mkArgZ (map Byte.repr (HMAC_SHA256.mkKey key)) Opad,
             Vptr cb (Int.add cofs (Int.repr 216)),
-            Vptr pb pofs, Tsh, 64, kv).
-      Now we need an extra semax_seq_skip before the forward_call' - but
-      such a semax_seq_skip is already contained in fwd_call', and we should be
-      in the semax _ _(Scall _ _ _ ) _ case.*)
- (* adding sth like this does not help  simpl; normalize. unfold POSTCONDITION, abbreviate. simpl; normalize.
-    Also: just call forward_call' worked fine at the corresponding place after the ipad loop (line 565 above)*)
-   rewrite -> semax_seq_skip.
-   Opaque firstn. 
-   forward_call' (init_s256abs, 
-            HMAC_SHA256.mkArgZ (map Byte.repr (HMAC_SHA256.mkKey key)) Opad,
-            Vptr cb (Int.add cofs (Int.repr 216)),
-            Vptr pb pofs, Tsh, 64, kv) opadSHAabs.
-    { assert (FR: Frame = [
-         (sha256state_ ipadSHAabs (Vptr cb (Int.add cofs (Int.repr 108))));
-         (field_at Tsh t_struct_hmac_ctx_st [StructField _key_length]
-              (if zlt 64 (Zlength key)
-               then Vint (Int.repr 32)
-               else Vint (Int.repr (Zlength key))) (Vptr cb cofs));
-         (data_at Tsh (nested_field_type2 t_struct_hmac_ctx_st [StructField _key])
-              (map Vint (map Int.repr (HMAC_SHA256.mkKey key)))
-               (Vptr cb (Int.add cofs
-                  (Int.repr (nested_field_offset2 t_struct_hmac_ctx_st [StructField _key])))));
+            Vptr pb pofs, Tsh, 64, kv)  opadSHAabs.
+    { assert (FR: Frame = [(sha256state_ ipadSHAabs (Vptr cb cIoff));
          (field_at Tsh t_struct_hmac_ctx_st [StructField _md_ctx] emptySha (Vptr cb cofs));
-         (data_at Tsh (tarray tuchar (Zlength key)) (map Vint (map Int.repr key)) (Vptr kb kofs))]). 
-        subst Frame. reflexivity.
-      rewrite FR. clear FR Frame. 
-      cancel. unfold data_block. rewrite ZLO.
-      entailer!. simpl; normalize.
-      apply andp_right. 
-        simpl. apply prop_right. apply isbyte_map_ByteUnsigned.
-      cancel.
+         (data_at Tsh (tarray tuchar 64) (map Vint (map Int.repr (HMAC_SHA256.mkKey key))) (Vptr ckb ckoff));
+         (data_at Tsh (tarray tuchar (Zlength key)) (map Vint (map Int.repr key)) (Vptr kb kofs))]).
+        subst Frame; reflexivity.
+      rewrite FR; clear FR Frame. 
+      cancel. unfold data_block.
+      entailer!. rewrite Zlength_correct, ZLO. simpl; normalize.
+      entailer!. apply isbyte_map_ByteUnsigned.
     }
     { clear Frame HeqPostResetBranch HeqIPADcont; subst OPADcont.
       rewrite Zlength_mkArgZ. repeat rewrite map_length. rewrite mkKey_length. 
@@ -758,18 +722,21 @@ forward_if PostResetBranch.
             repeat rewrite map_length. rewrite mkKey_length. simpl. omega. 
     Transparent firstn. 
 
-    subst PostResetBranch; entailer. unfold sha256state_; normalize. rename r into iUpd. rename x into oUpd.
-        apply (exp_right (ipadSHAabs,(iUpd,(opadSHAabs,oUpd)))). entailer.
+    subst PostResetBranch; entailer. unfold sha256state_; normalize.
+    rename r into iUpd. rename x into oUpd.
+        apply (exp_right ipadSHAabs).
+        apply (exp_right iUpd). 
+        apply (exp_right opadSHAabs).
+        apply (exp_right oUpd). entailer. unfold postResetHMS.  
         unfold data_block, initPostResetConditional. simpl.
-        rewrite ZLO. entailer!. cancel.
+        apply (exp_right emptySha).
+        (*rewrite ZLO.*) normalize.
+        apply (exp_right l). entailer. cancel.
         unfold_data_at 4%nat. cancel.
     rewrite (field_at_data_at Tsh t_struct_hmac_ctx_st [StructField _i_ctx]).
     rewrite (field_at_data_at Tsh t_struct_hmac_ctx_st [StructField _o_ctx]).
-    rewrite (field_at_data_at Tsh t_struct_hmac_ctx_st [StructField _key]).
     unfold field_address. rewrite <- Heqs, <- Heqs0. simpl. cancel.
-    destruct (field_compatible_dec t_struct_hmac_ctx_st [StructField _i_ctx]
-              (Vptr cb cofs)); try contradiction.
-    unfold  nested_field_type2, nested_field_offset2; simpl. cancel.
+    rewrite Zlength_correct, ZLO. cancel.
   }
   { (*ELSE*) 
     forward. subst. unfold initPostKeyNullConditional. entailer!. 
@@ -778,11 +745,13 @@ forward_if PostResetBranch.
     unfold hmacstate_PreInitNull, hmac_relate_PreInitNull; simpl.
     destruct h1; entailer.
     if_tac; entailer.
-    destruct H8 as [ii [KLi [KLunsig [SF [ISHA OSHA]]]]].
-    apply (exp_right (iSha, (iCtx r, (oSha, oCtx r)))).
-    entailer!. cancel.
+       apply (exp_right iSha). 
+       apply (exp_right (iCtx v)).
+       apply (exp_right oSha).
+       apply (exp_right (oCtx v)).
+       entailer. cancel. 
     unfold hmacstate_PreInitNull, hmac_relate_PreInitNull; simpl.
-    apply (exp_right r). apply (exp_right v).
-    entailer!. exists ii; eauto.  
-   } 
+    apply (exp_right v). apply (exp_right x).
+    entailer!.
+   }
 Qed.
