sha/verif_hmacADT_cleanup.v
@@ -18,33 +18,23 @@ Proof.
 start_function.
 name ctx' _ctx.
 unfold hmacstate_PostFinal, hmac_relate_PostFinal. normalize. intros hst. normalize. 
-apply semax_pre with (P':=
-  PROP (size_compatible t_struct_hmac_ctx_st c /\
-        align_compatible t_struct_hmac_ctx_st c)
-   LOCAL  (`(eq c) (eval_id _ctx);
-   `(eq KV) (eval_var sha._K256 (tarray tuint 64)))
-   SEP 
-   (`(data_at Tsh t_struct_hmac_ctx_st
-        (upd_reptype t_struct_hmac_ctx_st [StructField _md_ctx] hst
-           (default_val t_struct_SHA256state_st)) c))).
-  entailer. unfold data_at. simpl. normalize.
-normalize.
+assert_PROP (size_compatible t_struct_hmac_ctx_st c /\
+        align_compatible t_struct_hmac_ctx_st c).
+{ unfold data_at. entailer!. } 
+destruct H0 as [SC AC].
 
-forward_call (Tsh, c, sizeof t_struct_hmac_ctx_st, Int.zero).
+forward_call' (Tsh, c, sizeof t_struct_hmac_ctx_st, Int.zero) rv.
   { assert (FR: Frame = nil).  
       subst Frame. reflexivity.
     rewrite FR. clear FR Frame.
-    entailer.
+    entailer!.
     eapply derives_trans. apply data_at_data_at_.
-       (*reflexivity.*)
     rewrite <- memory_block_data_at_; try reflexivity.
-    entailer.
+    entailer!.
     assumption. 
   }
-after_call. subst retval0.
 forward.
-unfold data_block. rewrite Zlength_correct; simpl. entailer. 
-apply prop_right.
+unfold data_block. rewrite Zlength_correct; simpl. entailer!. 
 assert (isByte0:  isbyteZ 0). unfold isbyteZ; omega.
 apply (Forall_list_repeat _ _ (Z.to_nat (sizeof t_struct_hmac_ctx_st)) _ isByte0). 
 Qed.
