sha/verif_hmacADT_init_part1_5.v
@@ -1,0 +1,350 @@
+Require Import floyd.proofauto.
+Import ListNotations.
+Require sha.sha.
+Require Import sha.SHA256.
+Local Open Scope logic.
+
+Require Import sha.spec_sha.
+Require Import sha.sha_lemmas.
+Require Import sha.HMAC_functional_prog.
+Require Import sha.HMAC256_functional_prog.
+
+Require Import sha.hmac_NK.
+Require Import sha.vst_lemmas.
+Require Import sha.hmac_pure_lemmas.
+Require Import sha.hmac_common_lemmas.
+Require Import sha.spec_hmacADT.
+
+Definition initPostKeyNullConditional l r (c:val) (k: val) h key ctxkey: mpred:=
+  match k with
+    Vint z => if Int.eq z Int.zero
+              then if zeq r Z0 
+                   then (hmacstate_PreInitNull key h c) * (data_at_ Tsh (tarray tuchar 64) ctxkey)
+                   else FF
+              else FF
+  | Vptr b ofs => if zeq r 0 then FF 
+                  else EX ll:_, EX CONT:_,
+                      !!(Forall isbyteZ key /\ has_lengthK ll key /\ l = Vint(Int.repr ll)) &&
+                    ((data_at Tsh t_struct_hmac_ctx_st CONT c) *
+                     (data_at Tsh (tarray tuchar 64) (map Vint (map Int.repr (HMAC_SHA256.mkKey key)))
+                      ctxkey) *
+                     (data_at Tsh (tarray tuchar (Zlength key)) (map Vint (map Int.repr key))
+                      (Vptr b ofs)))
+  | _ => FF
+  end. 
+
+Lemma hmac_init_part1_5: forall
+(Espec : OracleKind)
+(kb : block)
+(kofs : int)
+(l : val)
+(key : list Z)
+(kv : val)
+(h1 : hmacabs)
+(ctx' : name _ctx)
+(key' : name _key)
+(len' : name _len)
+(pad : val)
+(ckb : block)
+(ckoff : int)
+(PostKeyNull : environ -> mpred)
+(ll : Z)
+(Ctx : reptype t_struct_hmac_ctx_st)
+(KL : has_lengthK ll key)
+(L : l = Vint (Int.repr ll))
+(cb : block)
+(cofs : int)
+(HeqPostKeyNull : PostKeyNull =
+                 EX  cb0 : block,
+                 (EX  cofs0 : int,
+                  (EX  r : Z,
+                   PROP  (Vptr cb cofs = Vptr cb0 cofs0 /\ (r = 0 \/ r = 1))
+                   LOCAL  (temp _reset (Vint (Int.repr r));
+                   lvar _ctx_key (tarray tuchar 64) (Vptr ckb ckoff);
+                   lvar _pad (tarray tuchar 64) pad;
+                   temp _ctx (Vptr cb cofs); temp _key (Vptr kb kofs);
+                   temp _len l; gvar sha._K256 kv)
+                   SEP  (`(data_at_ Tsh (tarray tuchar 64) pad);
+                   `(initPostKeyNullConditional l r (Vptr cb cofs)
+                       (Vptr kb kofs) h1 key (Vptr ckb ckoff));
+                   `(K_vector kv)))))
+(isbyte_key : Forall isbyteZ key)
+(PostIf_j_Len : environ -> mpred)
+(HeqPostIf_j_Len : PostIf_j_Len =
+                  EX  CONT : reptype t_struct_hmac_ctx_st,
+                  PROP  ()
+                  LOCAL  (temp _reset (Vint (Int.repr 1));
+                  lvar _ctx_key (tarray tuchar 64) (Vptr ckb ckoff);
+                  lvar _pad (tarray tuchar 64) pad; temp _ctx (Vptr cb cofs);
+                  temp _key (Vptr kb kofs); temp _len l; gvar sha._K256 kv)
+                  SEP  (`(data_at_ Tsh (tarray tuchar 64) pad);
+                  `(data_at Tsh t_struct_hmac_ctx_st CONT (Vptr cb cofs));
+                  `(data_at Tsh (tarray tuchar (Zlength key))
+                      (map Vint (map Int.repr key)) (Vptr kb kofs));
+                  `(data_at Tsh (tarray tuchar 64)
+                      (map Vint (map Int.repr (HMAC_SHA256.mkKey key)))
+                      (Vptr ckb ckoff)); `(K_vector kv)))
+(ge_64_l : typed_false tint
+            (force_val
+               (both_int
+                  (fun n1 n2 : int => Some (Val.of_bool (Int.lt n1 n2)))
+                  sem_cast_neutral sem_cast_neutral (Vint (Int.repr 64)) l))),
+semax
+  (initialized_list [_j; _reset]
+     (func_tycontext f_HMAC_Init HmacVarSpecs HmacFunSpecs))
+  (PROP  ()
+   LOCAL  (temp _j (Vint (Int.repr 64)); temp _reset (Vint (Int.repr 1));
+   lvar _ctx_key (tarray tuchar 64) (Vptr ckb ckoff);
+   lvar _pad (tarray tuchar 64) pad; temp _ctx (Vptr cb cofs);
+   temp _key (Vptr kb kofs); temp _len l; gvar sha._K256 kv)
+   SEP  (`(data_at Tsh t_struct_hmac_ctx_st Ctx (Vptr cb cofs));
+   `(data_at Tsh (tarray tuchar (Zlength key)) (map Vint (map Int.repr key))
+       (Vptr kb kofs)); `(data_at_ Tsh (tarray tuchar 64) pad);
+   `(data_at_ Tsh (tarray tuchar 64) (Vptr ckb ckoff)); `(K_vector kv)))
+  (Ssequence
+     (Scall None
+        (Evar _memcpy
+           (Tfunction
+              (Tcons (tptr tvoid) (Tcons (tptr tvoid) (Tcons tuint Tnil)))
+              (tptr tvoid) cc_default))
+        [Evar _ctx_key (tarray tuchar 64); Etempvar _key (tptr tuchar);
+        Etempvar _len tint])
+     (Scall None
+        (Evar _memset
+           (Tfunction (Tcons (tptr tvoid) (Tcons tint (Tcons tuint Tnil)))
+              (tptr tvoid) cc_default))
+        [Eaddrof
+           (Ederef
+              (Ebinop Oadd (Evar _ctx_key (tarray tuchar 64))
+                 (Etempvar _len tint) (tptr tuchar)) tuchar) (tptr tuchar);
+        Econst_int (Int.repr 0) tint;
+        Ebinop Osub (Econst_int (Int.repr 64) tuint) (Etempvar _len tint)
+          tuint])) (normal_ret_assert PostIf_j_Len).
+Proof. intros.
+  subst l. rename ll into l. destruct KL as [KL1 [KL2 KL3]].
+
+     (*call to memcpy*)
+     focus_SEP 1 3.
+     unfold data_at_. 
+(*     assert_PROP (isptr ctxkey). entailer!. 
+     apply isptrD in H; destruct H as [ckb [ckofs CTK]]; subst ctxkey. simpl.*)
+     assert_PROP  (offset_in_range 0 (Vptr ckb ckoff) /\ offset_in_range 64 (Vptr ckb ckoff)).
+     { entailer. 
+       specialize (split_offset_array_at 0 Tsh). unfold tarray. intros X.
+       rewrite X with (len:=64)(v:=Vptr ckb ckoff). entailer.
+       apply prop_right. specialize (Int.unsigned_range ckoff). intros x; omega.
+       reflexivity. rewrite Zlength_correct; simpl; omega. simpl; omega.
+     }
+     destruct H as [OIR0_328 OIR64_328].
+     
+     unfold tarray.
+     remember (64 - l) as l64.
+     assert (HH: match Zlength key with
+                     | 0 => 0
+                     | Z.pos y' => Z.pos y'
+                     | Z.neg y' => Z.neg y'
+                 end = Zlength key).
+     { destruct (Zlength key); reflexivity. }
+     forward_call' ((Tsh, Tsh), Vptr ckb ckoff, 
+             Vptr kb kofs, mkTrep (Tarray tuchar (Zlength key) noattr) 
+                     (map Vint (map Int.repr key))) v.
+     { apply prop_right. rewrite Z.max_r.
+       destruct (Zlength key); trivial. apply KL2. }
+     { assert (FR: Frame = [
+         (data_at Tsh (Tarray tuchar l64 noattr)
+             (Znth l [] Vundef :: skipn (nat_of_Z (l + 1)) [])
+             (offset_val (Int.repr l) (Vptr ckb ckoff)));
+         (data_at_ Tsh t_struct_hmac_ctx_st (Vptr cb cofs));
+         (data_at_ Tsh (Tarray tuchar 64 noattr) pad); (K_vector kv)]).
+         subst Frame; reflexivity.
+       rewrite FR; clear FR Frame.   
+       simpl; entailer!.
+         rewrite Zlength_max_zero, HH.
+         cancel.
+              rewrite (data_at_Tarray_split3a Tsh tuchar 64 noattr (Zlength key)). 2: omega.
+              specialize (split_offset_array_at (length key)). unfold tarray; intros SOA.
+              rewrite SOA; try reflexivity; clear SOA.
+              Focus 2. repeat rewrite Zlength_correct.
+                       repeat rewrite map_length. rewrite app_length.
+                       rewrite force_lengthn_length_n, nat_of_Z_of_nat; simpl.
+                       rewrite Nat2Z.inj_add. omega. 
+              2: rewrite Zlength_correct in ge_64_l; omega.
+        entailer. rewrite firstn_app1.
+              Focus 2. rewrite force_lengthn_length_n. trivial.
+              rewrite firstn_precise.
+              Focus 2. repeat rewrite map_length.  rewrite force_lengthn_length_n. trivial.
+        apply sepcon_derives. 
+         eapply derives_trans; try apply data_at_data_at_.
+               rewrite data_at__memory_block. entailer!.
+               simpl. rewrite <- Zlength_correct.
+               rewrite Zlength_max_zero, HH. cancel.
+               reflexivity.
+               simpl. rewrite <- Zlength_correct, Zlength_max_zero, HH. 
+               rewrite <- initialize.max_unsigned_modulus. specialize Int.max_signed_unsigned; omega.
+         
+              rewrite skipn_app2.
+              Focus 2. rewrite force_lengthn_length_n. omega.
+              rewrite force_lengthn_length_n.
+              assert (X: (length key - length key = 0)%nat). omega.
+              rewrite X, skipn_0, <- Zlength_correct.
+              unfold offset_val. cancel. 
+     } 
+     { simpl. rewrite Zlength_max_zero, HH. subst l. split; trivial.
+          rewrite int_max_unsigned_eq.
+          rewrite int_max_signed_eq in KL2. omega. }
+
+     simpl. subst v. remember (map Vint (map Int.repr key)) as KCONT.
+
+     (*call memset*)
+     clear HH.
+     forward_call' (Tsh, Vptr ckb (Int.add ckoff (Int.repr (Zlength key))), l64, Int.zero)
+       vret.
+     { rewrite <- KL1.
+       match goal with |- _ * _ * ?A * _ * _ * _ |-- _ => 
+                  pull_left A end.
+       repeat rewrite sepcon_assoc. apply sepcon_derives; [ | cancel].
+       eapply derives_trans; try apply data_at_data_at_.
+               rewrite data_at__memory_block. 
+               rewrite sizeof_Tarray. entailer!.
+       rewrite Zmax_spec. simpl in ge_64_l. apply typed_false_of_bool in ge_64_l.
+       rewrite if_false. trivial. subst l64 l. clear - KL2 ge_64_l. 
+           apply lt_false_inv in ge_64_l.
+           rewrite Int.signed_repr in ge_64_l.
+           2: rewrite int_min_signed_eq, int_max_signed_eq; omega.
+           rewrite Int.signed_repr in ge_64_l.
+           2: rewrite int_min_signed_eq; omega.
+           omega.
+       reflexivity.
+       subst l64.
+       rewrite  sizeof_Tarray.
+       change Int.modulus with (Int.max_unsigned+1).
+       repable_signed. 
+       apply Z.max_r. subst l. simpl in ge_64_l. apply typed_false_of_bool in ge_64_l. 
+           clear - KL2 ge_64_l. 
+           apply lt_false_inv in ge_64_l.
+           rewrite Int.signed_repr in ge_64_l.
+           2: rewrite int_min_signed_eq, int_max_signed_eq; omega.
+           rewrite Int.signed_repr in ge_64_l.
+           2: rewrite int_min_signed_eq; omega.
+           omega. 
+     } 
+     { split; auto. subst l64 l.  simpl in ge_64_l. apply typed_false_of_bool in ge_64_l. 
+           clear - KL2 ge_64_l. 
+           apply lt_false_inv in ge_64_l.
+           rewrite Int.signed_repr in ge_64_l.
+           2: rewrite int_min_signed_eq, int_max_signed_eq; omega.
+           rewrite Int.signed_repr in ge_64_l.
+           2: rewrite int_min_signed_eq; omega. split. omega. 
+           rewrite int_max_unsigned_eq; omega. }
+
+     subst PostIf_j_Len.
+     entailer!.
+     destruct (zlt 64 (Zlength key)). omega. rewrite Zlength_correct in g. apply (Nat2Z.inj_ge 64) in g.
+     clear H0 TC0 h1.
+     remember (64 - Zlength key) as ZK64.
+     rewrite (data_at_Tarray_split3a Tsh tuchar 64 noattr (Zlength key)). 2: omega.
+              simpl. unfold nat_of_Z. rewrite Zlength_correct, Nat2Z.id.
+              rewrite sepcon_comm.
+              specialize (split_offset_array_at (length key) Tsh tuchar 64). unfold tarray; intros SOA.
+              rewrite SOA; try reflexivity; clear SOA.
+      2: rewrite Zlength_correct, app_length, force_lengthn_length_n, Nat2Z.inj_add; omega.
+      2: rewrite Zlength_correct in ge_64_l; omega.
+      assert (STO: sizeof tuchar = 1) by reflexivity. rewrite STO, Z.mul_1_l. rewrite Z.mul_1_l.
+      entailer!. 
+
+     remember (64 - Zlength key) as ZK64. 
+      specialize (split_offset_array_at (Z.to_nat ZK64) Tsh tuchar ZK64). intros X. unfold tarray in X. 
+        rewrite X. clear X. entailer!.
+     remember (64 - Zlength key) as ZK64. 
+     assert (F64: false = (Zlength key >? 64)). 
+     { rewrite Z.gtb_ltb. symmetry. apply Fcore_Zaux.Zlt_bool_false. omega. }
+     rewrite firstn_app1. 2: rewrite force_lengthn_length_n; trivial.
+     rewrite firstn_precise. 2: rewrite length_list_repeat; trivial.
+     rewrite firstn_precise. 2: rewrite force_lengthn_length_n; trivial.
+     assert (NULL: ZK64 - Z.of_nat (Z.to_nat ZK64) = 0).
+     { rewrite Z2Nat.id. omega. omega. }
+     rewrite NULL.
+     rewrite skipn_short. 2: rewrite length_list_repeat; omega.
+
+     apply (exp_right (default_val t_struct_hmac_ctx_st)). 
+     entailer. cancel. 
+     remember (64 - Z.of_nat (length key)). 
+     remember (Z.of_nat (Z.to_nat (64 - Zlength key))). 
+     remember (Z.to_nat (64 - Zlength key)). simpl.
+     apply derives_trans with
+       (Q:= data_at Tsh (Tarray tuchar (Z.of_nat (length key)) noattr)
+               (map Vint (map Int.repr key)) (Vptr ckb ckoff) *
+            data_at Tsh (Tarray tuchar z0 noattr) (list_repeat n (Vint Int.zero))
+              (Vptr ckb (Int.add ckoff (Int.repr (Z.of_nat (length key)))))).
+     { cancel. 
+       eapply derives_trans; try apply data_at_data_at_.
+       rewrite data_at__memory_block. simpl. entailer!.
+       reflexivity. simpl.
+       specialize Int.modulus_pos. omega.
+     }
+     { apply sepcon_derives.
+       { apply data_at_Tarray_ext_derives. intros i I.
+         apply data_at_triv. unfold Znth. if_tac. trivial. clear H15.
+         rewrite nth_force_lengthn.
+         Focus 2. split. omega. destruct I as [Ipos I]. apply Z2Nat.inj_lt in I; trivial.
+                  rewrite Nat2Z.id in I. trivial. omega.
+         assert (Z32: (Z.to_nat i < length key)%nat).
+                  clear - I; destruct I as [XX YY]. rewrite Z2Nat.inj_lt in YY.
+                  rewrite Nat2Z.id in YY; trivial. trivial. omega. 
+         apply eq_sym.
+         assert (L1: (Z.to_nat i < length (HMAC_SHA256.mkKey key))%nat).
+           rewrite mkKey_length; unfold SHA256.BlockSize.
+           assert (Zlength key <= 64) by omega. apply Z2Nat.inj_le in H15. simpl in H15.
+           rewrite Zlength_correct, Nat2Z.id in H15. omega.
+           omega. omega.
+         rewrite nth_map' with (d':=Int.zero).
+         rewrite nth_map' with (d':=Int.zero).
+         rewrite nth_map' with (d':=Z0); trivial.
+         rewrite nth_map' with (d':=Z0); trivial. f_equal. f_equal.         
+         eapply mkKey_left; trivial. rewrite Zlength_correct. trivial.
+         rewrite map_length; trivial. rewrite map_length; trivial.
+       }
+       { unfold offset_val. rewrite skipn_force_lengthn_app. 
+         simpl. specialize (Nat2Z.inj_add (length key) 1). simpl; intros ZZ. rewrite <- ZZ. clear ZZ. 
+         rewrite Nat2Z.id. (*Z2Nat.id*)
+         (*rewrite HeqZK64, Zlength_correct.*)
+         assert (z = z0). subst. rewrite Z2Nat.id, Zlength_correct; trivial. omega.
+         rewrite <- H15 in *. clear H15 Heqz0.
+         apply data_at_Tarray_ext_derives.
+         assert (z = Z.of_nat n).
+            subst. rewrite Z2Nat.id, Zlength_correct; trivial. omega.
+         clear Heqz. subst z. subst n. rewrite Z2Nat.id, Zlength_correct. 2: omega.
+         intros i I.
+         apply data_at_triv. unfold Znth. if_tac. trivial. clear H15.
+         destruct (zlt (Z.of_nat (length key)) 0).
+         rewrite <- Zlength_correct in l. omega.
+         rewrite nth_indep with (d:=(default_val tuchar))(d':=Vint (Int.repr 0)).
+         Focus 2. rewrite length_list_repeat. apply Z2Nat.inj_lt. omega. omega. omega. 
+         rewrite nth_list_repeat. (* rewrite HeqZK64, Zlength_correct in I.*)
+         remember (Z.to_nat i) as K; destruct K; simpl.
+         rewrite nth_map' with (d':=Int.zero).
+         rewrite nth_map' with (d':=Z0); trivial. f_equal. f_equal.    
+         rewrite mkKey_right; trivial. rewrite Zlength_correct. omega.
+         rewrite mkKey_length, Nat2Z.id. unfold SHA256.BlockSize. omega.
+         rewrite map_length, mkKey_length, Nat2Z.id. unfold SHA256.BlockSize. omega.
+         rewrite nth_skipn. 
+         assert (KK: (K + (length key + 1) = Z.to_nat (Z.of_nat (length key) + i))%nat).
+            rewrite Z2Nat.inj_add. (*rewrite Z2Nat.inj_add.*) rewrite <- HeqK.
+            rewrite Nat2Z.id. omega. omega. omega. (*
+            remember (Z.to_nat (Z.of_nat (length key))) as u. simpl. rewrite <- plus_n_Sm. rewrite <- (plus_Snm_nSm u). omega.
+            rewrite <- Zlength_correct. apply Zlength_nonneg.
+            omega.
+            rewrite <- Zlength_correct. apply Zlength_nonneg.
+            omega.*)
+         rewrite KK; clear KK.
+         rewrite nth_map' with (d':=Int.zero).
+         rewrite nth_map' with (d':=Z0); trivial. f_equal. f_equal. 
+         rewrite mkKey_right; trivial. rewrite Zlength_correct. omega.
+         rewrite mkKey_length. unfold SHA256.BlockSize. apply (Z2Nat.inj_lt _ 64). omega. omega. omega. 
+         rewrite map_length. rewrite mkKey_length. unfold SHA256.BlockSize. apply (Z2Nat.inj_lt _ 64). omega. omega. omega. 
+       }
+     } 
+     { reflexivity. }
+     { rewrite Zlength_correct, length_list_repeat. omega. }
+     { rewrite Z2Nat.id; omega. }
+Qed.
