sha/verif_hmacNK_cleanup.v
@@ -20,22 +20,21 @@ name ctx' _ctx.
 unfold hmacstate_PostFinal, hmac_relate_PostFinal. normalize. intros hst. normalize.
 assert_PROP (size_compatible t_struct_hmac_ctx_st c /\
         align_compatible t_struct_hmac_ctx_st c).
-{ unfold data_at. entailer. } 
+{ unfold data_at. entailer!. } 
 destruct H0 as [SC AC].
 
 forward_call' (Tsh, c, sizeof t_struct_hmac_ctx_st, Int.zero) rv.
   { assert (FR: Frame = nil).  
       subst Frame. reflexivity.
     rewrite FR. clear FR Frame.
-    entailer.
+    entailer!.
     eapply derives_trans. apply data_at_data_at_.
     rewrite <- memory_block_data_at_; try reflexivity.
-    entailer.
+    entailer!.
     assumption. 
   }
 forward.
-unfold data_block. rewrite Zlength_correct; simpl. entailer. 
-apply prop_right.
+unfold data_block. rewrite Zlength_correct; simpl. entailer!. 
 assert (isByte0:  isbyteZ 0). unfold isbyteZ; omega.
 apply (Forall_list_repeat _ _ (Z.to_nat (sizeof t_struct_hmac_ctx_st)) _ isByte0). 
 Qed.
