sha/verif_hmacNK_crypto.v
@@ -101,7 +101,7 @@ rename H into WrshMD.
 rewrite memory_block_isptr. normalize.
 (*NEW: crypto proof requires that we first extract isbyteZ key*)
 assert_PROP (Forall isbyteZ key).
-  entailer.
+  entailer!.
 rename H2 into isbyteZ_Key.
 rename H into isPtrMD. rename H0 into KL. rename H1 into DL.
 
@@ -113,13 +113,13 @@ forward_if  (
    SEP  (`(data_at_ Tsh t_struct_hmac_ctx_st c); `(data_block Tsh key k);
    `(data_block Tsh data d); `(K_vector kv);
    `(memory_block shmd (Int.repr 32) md))).
-  { (* Branch1 *) exfalso. subst md. contradiction.  }
-  { (* Branch2 *) forward. entailer. } 
+  { (* Branch1 *) inv H. }
+  { (* Branch2 *) forward. entailer!. } 
 normalize. rename H into isptrC.
 
 remember (HMACabs init_s256abs init_s256abs init_s256abs) as dummyHMA.
 forward_call' (c, k, kl, key, kv, dummyHMA) h.
-  { unfold initPre. entailer.
+  { unfold initPre. entailer!.
     apply isptrD in Pk. destruct Pk as [kb [kofs HK]]. rewrite HK.
     cancel.
   }
