sha/verif_hmacNK_final.v
@@ -15,18 +15,13 @@ Require Import sha.vst_lemmas.
 Require Import hmac_pure_lemmas.
 Require Import hmac_common_lemmas.
 
-Lemma withspacer_refl: forall sh a P, withspacer sh a a P = P.
-Proof. intros. unfold withspacer. 
-  rewrite <- Zminus_diag_reverse. trivial.
-Qed.
-
 Lemma body_hmac_final: semax_body HmacVarSpecs HmacFunSpecs 
        f_HMAC_Final HMAC_Final_spec.
 Proof.
 start_function.
 name ctx' _ctx.
 name md' _md.
-simpl_stackframe_of. fixup_local_var; intro b.
+simpl_stackframe_of. fixup_local_var; intro buf.
 
 rename H into WrshMD. 
 rewrite memory_block_isptr. unfold hmacstate_. normalize.
@@ -38,7 +33,7 @@ destruct H as [reprMD [reprI [reprO [iShaLen oShaLen]]]].
 unfold_data_at 1%nat.
 rewrite field_at_data_at with (gfs:=[StructField _md_ctx]).
 assert_PROP (isptr (field_address t_struct_hmac_ctx_st [StructField _md_ctx] c)).
-{ entailer. }
+{ entailer!. }
 apply isptrD in H; destruct H as [cb [coff COff]]. rewrite COff in *.
 unfold field_address in COff.
 remember (field_compatible_dec t_struct_hmac_ctx_st [StructField _md_ctx]
@@ -49,43 +44,42 @@ unfold nested_field_offset2, offset_val in COff. simpl in  COff.
 destruct c; inversion COff; clear COff. rewrite Int.add_zero in H1. subst cb coff.
 
 rewrite <- memory_block_data_at_ ; try reflexivity.
-Focus 2. red. destruct b; trivial. simpl. apply Z.divide_1_l.
+Focus 2. red. destruct buf; trivial. simpl. apply Z.divide_1_l.
 
 (*Call Sha_Final*)
-forward_call' (ctx, b, Vptr b0 i, Tsh, kv).
+forward_call' (ctx, buf, Vptr b i, Tsh, kv).
   { assert (FR: Frame = [
      (field_at Tsh t_struct_hmac_ctx_st [StructField _o_ctx]
-       (snd (snd ST))  (Vptr b0 i));
-     (field_at Tsh t_struct_hmac_ctx_st [StructField _i_ctx] (fst (snd ST)) (Vptr b0 i));
+       (snd (snd ST))  (Vptr b i));
+     (field_at Tsh t_struct_hmac_ctx_st [StructField _i_ctx] (fst (snd ST)) (Vptr b i));
        (memory_block shmd (Int.repr 32) md)]).
        subst Frame. reflexivity.
     rewrite FR. clear FR Frame. 
-    entailer. cancel.
-    unfold sha256state_. apply exp_right with (x:= mdCtx ST). entailer.
+    entailer!. cancel.
+    unfold sha256state_. apply (exp_right (mdCtx ST)). entailer!.
   }
 normalize. simpl.
 
 eapply semax_pre with (P':=(PROP  ()
-   LOCAL  (lvar _buf (tarray tuchar 32) b; temp _md md;
-   temp _ctx (Vptr b0 i); gvar sha._K256 kv)
+   LOCAL  (lvar _buf (tarray tuchar 32) buf; temp _md md;
+   temp _ctx (Vptr b i); gvar sha._K256 kv)
    SEP  (`(K_vector kv); 
-   `(data_at Tsh t_struct_hmac_ctx_st (default_val sha.t_struct_SHA256state_st, snd ST) (Vptr b0 i));
-   `(data_block Tsh (sha_finish ctx) b);
+   `(data_at Tsh t_struct_hmac_ctx_st (default_val sha.t_struct_SHA256state_st, snd ST) (Vptr b i));
+   `(data_block Tsh (sha_finish ctx) buf);
    `(memory_block shmd (Int.repr 32) md)))).
-{ entailer. 
+{ entailer!. 
       unfold_data_at 1%nat. simpl. cancel. unfold data_at_.
       rewrite (field_at_data_at Tsh t_struct_hmac_ctx_st [StructField _md_ctx]); try reflexivity.
-      unfold nested_field_type2, nested_field_offset2, field_address; simpl. rewrite <- Heqs. simpl. entailer.
+      unfold nested_field_type2, nested_field_offset2, field_address; simpl. rewrite <- Heqs. simpl. entailer!.
 }
 
 unfold_data_at 1%nat.
 rewrite (field_at_data_at _ _ [StructField _o_ctx]); try reflexivity.
-(*new: extract info from field_address as early as possible*)
-assert_PROP (isptr (field_address t_struct_hmac_ctx_st [StructField _o_ctx] (Vptr b0 i))).
-  entailer.
+assert_PROP (isptr (field_address t_struct_hmac_ctx_st [StructField _o_ctx] (Vptr b i))).
+  entailer!.
 apply isptrD in H; destruct H as [? [? OCTX]]; rewrite OCTX.
 unfold field_address in OCTX.
-destruct (field_compatible_dec t_struct_hmac_ctx_st [StructField _o_ctx] (Vptr b0 i));
+destruct (field_compatible_dec t_struct_hmac_ctx_st [StructField _o_ctx] (Vptr b i));
    inversion OCTX; clear OCTX. 
 subst x x0.
 rename f0 into FCO.
@@ -94,8 +88,8 @@ unfold field_address. simpl. rewrite <- Heqs.
 unfold nested_field_type2; simpl.
 unfold nested_field_offset2; simpl. 
 
-replace_SEP 2 `(memory_block Tsh (Int.repr (sizeof (nested_field_type2 t_struct_hmac_ctx_st [StructField _md_ctx]))) ((Vptr b0 i))).
-  { entailer. 
+replace_SEP 2 `(memory_block Tsh (Int.repr (sizeof (nested_field_type2 t_struct_hmac_ctx_st [StructField _md_ctx]))) ((Vptr b i))).
+  { entailer!. 
     eapply derives_trans. apply data_at_data_at_.
     rewrite <- (memory_block_data_at_ Tsh (nested_field_type2 t_struct_hmac_ctx_st [StructField _md_ctx])).
     unfold nested_field_type2; simpl. cancel.
@@ -106,8 +100,8 @@ replace_SEP 2 `(memory_block Tsh (Int.repr (sizeof (nested_field_type2 t_struct_
   }
 
 destruct ST as [MD [iCTX oCTX]]. simpl in *.
-forward_call' (Tsh, Tsh, Vptr b0 i, offset_val
-          (Int.repr (nested_field_offset2 t_struct_hmac_ctx_st [StructField _o_ctx])) (Vptr b0 i), 
+forward_call' (Tsh, Tsh, Vptr b i, offset_val
+          (Int.repr (nested_field_offset2 t_struct_hmac_ctx_st [StructField _o_ctx])) (Vptr b i), 
           (mkTrep t_struct_SHA256state_st oCTX)) rv.
 subst rv; simpl. 
 
@@ -117,17 +111,17 @@ assert (SFL: Zlength (sha_finish ctx) = 32).
 
 (*Call sha256Update*)
 Opaque firstn.
-forward_call' (oSha, sha_finish ctx, Vptr b0 i, b, Tsh, Z.of_nat SHA256.DigestLength, kv) updSha.
+forward_call' (oSha, sha_finish ctx, Vptr b i, buf, Tsh, Z.of_nat SHA256.DigestLength, kv) updSha.
   { assert (FR: Frame = [
        (data_at Tsh t_struct_SHA256state_st oCTX
-           (offset_val (Int.repr (nested_field_offset2 t_struct_hmac_ctx_st [StructField _o_ctx])) (Vptr b0 i)));
-       (field_at Tsh t_struct_hmac_ctx_st [StructField _i_ctx] iCTX (Vptr b0 i));
+           (offset_val (Int.repr (nested_field_offset2 t_struct_hmac_ctx_st [StructField _o_ctx])) (Vptr b i)));
+       (field_at Tsh t_struct_hmac_ctx_st [StructField _i_ctx] iCTX (Vptr b i));
        (memory_block shmd (Int.repr 32) md)]).
        subst Frame; reflexivity.
     rewrite FR; clear FR Frame. 
-    entailer. cancel.
+    entailer!. cancel.
     unfold sha256state_. apply (exp_right oCTX).
-    entailer.
+    entailer!.
   }
   { unfold SHA256.DigestLength. 
     rewrite oShaLen. simpl. simpl. split. omega. split. 
@@ -142,17 +136,17 @@ Focus 2. eapply Zlength_length in SFL. apply SFL. omega.
 unfold sha256state_. normalize. intros updShaST. normalize. rename H into updShaREL. 
 
 (*Call SHA_Final*)
-forward_call' (updSha, md, Vptr b0 i, shmd, kv).
-  { assert (FR: Frame = [ (data_block Tsh (sha_finish ctx)  b);
+forward_call' (updSha, md, Vptr b i, shmd, kv).
+  { assert (FR: Frame = [ (data_block Tsh (sha_finish ctx) buf);
       (data_at Tsh t_struct_SHA256state_st oCTX
-         (offset_val (Int.repr (nested_field_offset2 t_struct_hmac_ctx_st [StructField _o_ctx])) (Vptr b0 i)));
-      (field_at Tsh t_struct_hmac_ctx_st [StructField _i_ctx] iCTX (Vptr b0 i))]).
+         (offset_val (Int.repr (nested_field_offset2 t_struct_hmac_ctx_st [StructField _o_ctx])) (Vptr b i)));
+      (field_at Tsh t_struct_hmac_ctx_st [StructField _i_ctx] iCTX (Vptr b i))]).
        subst Frame; reflexivity.
     rewrite FR; clear FR Frame. 
-    entailer. 
+    entailer!. 
     cancel.
     unfold sha256state_. 
-    apply (exp_right updShaST). entailer.
+    apply (exp_right updShaST). entailer!.
   }
 simpl.
 
@@ -167,22 +161,22 @@ cancel.
 unfold data_block.
 normalize.
 apply derives_trans with (Q:= hmacstate_PostFinal (HMACabs updSha iSha oSha)
-      (Vptr b0 i) *
+      (Vptr b i) *
     data_at Tsh (tarray tuchar 32) (map Vint (map Int.repr (sha_finish ctx)))
   (eval_lvar _buf (tarray tuchar 32) rho)).
 2: cancel.
 rewrite SFL in *. 
-rewrite lvar_eval_lvar with (v:=b); trivial. cancel.
-unfold hmacstate_PostFinal, hmac_relate_PostFinal. entailer.
+rewrite lvar_eval_lvar with (v:=buf); trivial. cancel.
+unfold hmacstate_PostFinal, hmac_relate_PostFinal. entailer!.
 apply (exp_right (updShaST, (iCTX, oCTX))).
 simpl. normalize.
 unfold_data_at 3%nat.
 cancel.
 rewrite (field_at_data_at _ _ [StructField _o_ctx]); try reflexivity.
 rewrite (field_at_data_at _ _ [StructField _md_ctx]); try reflexivity.
-entailer. unfold nested_field_type2; simpl.
+entailer!. unfold nested_field_type2; simpl.
 unfold field_address. rewrite <- Heqs.
 destruct (field_compatible_dec t_struct_hmac_ctx_st [StructField _o_ctx]
-            (Vptr b0 i)); try contradiction.
-unfold nested_field_offset2; simpl. rewrite Int.add_zero. entailer.
+            (Vptr b i)); try contradiction.
+unfold nested_field_offset2; simpl. rewrite Int.add_zero. entailer!.
 Qed.
