sha/verif_hmacNK_init_part1.v
@@ -165,21 +165,22 @@ forward_if PostKeyNull.
     simpl.  
     unfold force_val2, force_val1 in H; simpl in H. 
     unfold initPre. 
-    destruct k; try solve [eapply semax_pre; try eapply semax_ff; entailer].
+    destruct k; try solve [eapply semax_pre; try eapply semax_ff; entailer!].
     (*key' is integer, ie Null*)
-      remember (Int.eq i Int.zero) as d.
+    { remember (Int.eq i Int.zero) as d.
       destruct d; try solve [eapply semax_pre; try eapply semax_ff; entailer].
       apply binop_lemmas.int_eq_true in Heqd. simpl in *. subst i.
-      unfold Int.zero in *. simpl in *. inversion H.
+      unfold Int.zero in *. simpl in *. inversion H. }
     (*key' is ptr*)
     normalize. clear H.
-    assert_PROP (isptr c). entailer. apply isptrD in H. destruct H as [cb [cofs CC]]; subst c.
+    assert_PROP (isptr c). { entailer!. }
+    apply isptrD in H. destruct H as [cb [cofs CC]]; subst c.
     rename b into kb; rename i into kofs.
     assert_PROP (Forall isbyteZ key).
-      { unfold data_block. entailer. }
+      { unfold data_block. entailer!. }
     rename H into isbyte_key. 
     replace_SEP 1 (`(data_at Tsh (tarray tuchar (Zlength key)) (map Vint (map Int.repr key)) (Vptr kb kofs))).
-       unfold data_block. entailer.
+       unfold data_block. entailer!.
 
     forward v. subst v. 
     forward. (*j=HMAC_MAX_MD_CBLOCK*)
@@ -213,7 +214,7 @@ forward_if PostKeyNull.
       (*new: extract info from field_address as early as possible*)
       assert_PROP (isptr (field_address t_struct_hmac_ctx_st [StructField _md_ctx]
                           (Vptr cb cofs))).
-      { entailer. }
+      { entailer!. }
       apply isptrD in H; destruct H as [? [? PT]]; rewrite PT.
       unfold field_address in PT.
       destruct (field_compatible_dec t_struct_hmac_ctx_st [StructField _md_ctx]
@@ -251,7 +252,7 @@ forward_if PostKeyNull.
           subst Frame; reflexivity.
         rewrite FR; clear FR Frame.  
         unfold data_block. rewrite Zlength_correct. 
-        entailer. 
+        entailer!. 
       }
       { clear Frame HeqPostIf_j_Len HeqPostKeyNull.
         subst l. split. omega. 
@@ -270,16 +271,16 @@ forward_if PostKeyNull.
                subst l. rewrite Zlength_correct, Nat2Z.id. omega.
 
       replace_SEP 3 (`emp). 
-      { entailer.
+      { entailer!.
         rewrite Zlength_correct. rewrite Z.sub_diag.
         eapply derives_trans; try eapply data_at_data_at_.
              rewrite data_at__memory_block.
-               rewrite memory_block_zero_Vptr. entailer.
+               rewrite memory_block_zero_Vptr. entailer!.
                reflexivity. simpl; omega.
       }
 
      (*call Final*)
-(*     assert_PROP(isptr ctxkey). entailer.
+(*     assert_PROP(isptr ctxkey). entailer!.
      apply isptrD in H; destruct H as [ckb [ckoff X]]; subst ctxkey.*)
      rewrite (data_at_Tarray_split3 Tsh tuchar 64 noattr 32). 2: omega.
      simpl.
@@ -300,59 +301,59 @@ forward_if PostKeyNull.
           data_at_ Tsh (Tarray tuchar 64 noattr) pad]).
          subst Frame; reflexivity.
        rewrite FR; clear FR Frame.   
-       entailer. cancel.
+       entailer!. cancel.
        eapply derives_trans; try apply data_at_data_at_.
-               rewrite data_at__memory_block. entailer.
+               rewrite data_at__memory_block. entailer!.
                reflexivity. simpl; omega.
      }
      normalize.
 
      (*call memset*) 
      replace_SEP 3 (`(memory_block Tsh (Int.repr 32) (offset_val (Int.repr 32) (Vptr ckb ckoff)))).
-     { entailer. eapply derives_trans; try apply data_at_data_at_.
-       rewrite data_at__memory_block. entailer.
+     { entailer!. eapply derives_trans; try apply data_at_data_at_.
+       rewrite data_at__memory_block. entailer!.
        reflexivity. simpl. omega.
      }
      forward_call' (Tsh, offset_val (Int.repr 32) (Vptr ckb ckoff), 32, Int.zero)
         vret.
-     {subst PostIf_j_Len.
-      unfold data_block.
-      entailer!.
-    unfold_data_at 3%nat. cancel.
-     assert (SFL: Zlength  (sha_finish ctxSha) = 32).
-        destruct ctxSha. simpl. rewrite <- functional_prog.SHA_256'_eq, Zlength_correct, length_SHA256'. reflexivity. 
-     rewrite SFL.   
-     rewrite (field_at_data_at Tsh t_struct_hmac_ctx_st [StructField _md_ctx]); try reflexivity.
-      simpl. 
-     rewrite field_address_clarify by auto.
-     unfold nested_field_type2, nested_field_offset2. simpl.
-     normalize. cancel.
-     unfold tarray. rewrite (data_at_Tarray_split3 Tsh tuchar 64 noattr 32) by omega.
-     specialize (split_offset_array_at 32). unfold tarray; intros SOA.
-     rewrite SOA with (len :=64)(v:=Vptr ckb ckoff); try reflexivity; clear SOA.
+     { subst PostIf_j_Len.
+       unfold data_block.
+       entailer!.
+       unfold_data_at 3%nat. cancel.
+       assert (SFL: Zlength  (sha_finish ctxSha) = 32).
+       { destruct ctxSha. simpl. rewrite <- functional_prog.SHA_256'_eq, Zlength_correct, length_SHA256'. reflexivity. } 
+       rewrite SFL.   
+       rewrite (field_at_data_at Tsh t_struct_hmac_ctx_st [StructField _md_ctx]); try reflexivity.
+       simpl. 
+       rewrite field_address_clarify by auto.
+       unfold nested_field_type2, nested_field_offset2. simpl.
+       normalize. cancel.
+       unfold tarray. rewrite (data_at_Tarray_split3 Tsh tuchar 64 noattr 32) by omega.
+       specialize (split_offset_array_at 32). unfold tarray; intros SOA.
+       rewrite SOA with (len :=64)(v:=Vptr ckb ckoff); try reflexivity; clear SOA.
        Focus 2. rewrite Zlength_correct, app_length, force_lengthn_length_n, Nat2Z.inj_add, nat_of_Z_eq.
                 assert (HZ: Z.of_nat 32=32) by reflexivity. rewrite HZ; clear HZ. omega.
                 omega.
        2: simpl; omega.
-     entailer.
-     apply andp_right. apply prop_right. split; rewrite Zplus_0_r; trivial.
-     rewrite firstn_app1.
-     Focus 2. rewrite force_lengthn_length_n. simpl; omega. 
-     rewrite firstn_same. 
-     Focus 2. rewrite force_lengthn_length_n. simpl; omega. 
+       entailer.
+       apply andp_right. apply prop_right. split; rewrite Zplus_0_r; trivial.
+       rewrite firstn_app1.
+       Focus 2. rewrite force_lengthn_length_n. simpl; omega. 
+       rewrite firstn_same. 
+       Focus 2. rewrite force_lengthn_length_n. simpl; omega. 
 (*     assert (LengthShaFinish: Zlength (sha_finish ctxSha) = 32).
                  unfold sha_finish. destruct ctxSha.
         rewrite <- functional_prog.SHA_256'_eq, Zlength_correct, length_SHA256'. reflexivity.
      rewrite LengthShaFinish. *)
-     assert (NZ: nat_of_Z 32 = 32%nat) by reflexivity. rewrite NZ; clear NZ.
-     rewrite skipn_force_lengthn_app.
-     assert (SF:64 - Z.of_nat 32 = 32) by reflexivity. rewrite SF; clear SF.
-     rewrite sepcon_comm. 
-     apply sepcon_derives. 
-     { apply data_at_Tarray_ext_derives. intros. 
+       assert (NZ: nat_of_Z 32 = 32%nat) by reflexivity. rewrite NZ; clear NZ.
+       rewrite skipn_force_lengthn_app.
+       assert (SF:64 - Z.of_nat 32 = 32) by reflexivity. rewrite SF; clear SF.
+       rewrite sepcon_comm. 
+       apply sepcon_derives. 
+       { apply data_at_Tarray_ext_derives. intros. 
               unfold Znth. if_tac. omega.
               assert (Z32: (Z.to_nat i < 32)%nat).
-                  clear - H; destruct H as [XX YY]. rewrite Z2Nat.inj_lt in YY.
+                  clear - H10; destruct H10 as [XX YY]. rewrite Z2Nat.inj_lt in YY.
                   apply YY. omega. omega.
          apply data_at_triv.
          rewrite nth_force_lengthn. 2: simpl; omega.
@@ -365,18 +366,18 @@ forward_if PostKeyNull.
               unfold HMAC_SHA256.zeroPad.
               rewrite <- functional_prog.SHA_256'_eq.
               rewrite app_nth1. inversion updAbs. subst. clear updAbs. simpl in *.
-                      rewrite <- H15. trivial.
+                      rewrite <- H21. trivial.
               rewrite length_SHA256'; trivial.
               repeat rewrite map_length. rewrite mkKey_length; unfold SHA256.BlockSize; simpl. omega.
               repeat rewrite map_length. unfold sha_finish. inversion updAbs. rewrite <- functional_prog.SHA_256'_eq, length_SHA256'. trivial.
        }
-     { apply data_at_Tarray_ext_derives. intros. 
-       unfold Znth. if_tac. omega. if_tac. omega. clear H5 H6. 
-       apply data_at_triv.
-       assert (Z32: (Z.to_nat i < 32)%nat).
-                  clear - H; destruct H as [XX YY]. rewrite Z2Nat.inj_lt in YY.
+       { apply data_at_Tarray_ext_derives. intros. 
+         unfold Znth. if_tac. omega. if_tac. omega. clear H5 H6. 
+         apply data_at_triv.
+         assert (Z32: (Z.to_nat i < 32)%nat).
+                  clear - H10; destruct H10 as [XX YY]. rewrite Z2Nat.inj_lt in YY.
                   apply YY. omega. omega.
-       unfold HMAC_SHA256.mkKey. 
+         unfold HMAC_SHA256.mkKey. 
                assert (Kgt: Zlength key > Z.of_nat SHA256.BlockSize).  simpl; omega.
                apply Zgt_is_gt_bool in Kgt.
                rewrite Kgt. unfold HMAC_SHA256.zeroPad. repeat rewrite map_app.
@@ -403,16 +404,16 @@ forward_if PostKeyNull.
                 rewrite length_list_repeat. omega. 
                 rewrite map_length, length_list_repeat. omega. 
                 unfold SHA256.DigestLength. simpl; omega.
-         }
+       }
+     }
    }
-}
    { (* j >= len*)
      rename H into ge_64_l. 
 
      (*call to memcpy*)
      focus_SEP 1 3.
      unfold data_at_. 
-(*     assert_PROP (isptr ctxkey). entailer. 
+(*     assert_PROP (isptr ctxkey). entailer!. 
      apply isptrD in H; destruct H as [ckb [ckofs CTK]]; subst ctxkey. simpl.*)
      assert_PROP  (offset_in_range 0 (Vptr ckb ckoff) /\ offset_in_range 64 (Vptr ckb ckoff)).
      { entailer. 
@@ -444,7 +445,7 @@ forward_if PostKeyNull.
          (data_at_ Tsh (Tarray tuchar 64 noattr) pad); (K_vector kv)]).
          subst Frame; reflexivity.
        rewrite FR; clear FR Frame.   
-       simpl; entailer.
+       simpl; entailer!.
          rewrite Zlength_max_zero, HH.
          cancel.
               rewrite (data_at_Tarray_split3a Tsh tuchar 64 noattr (Zlength key)). 2: omega.
@@ -461,7 +462,7 @@ forward_if PostKeyNull.
               Focus 2. repeat rewrite map_length.  rewrite force_lengthn_length_n. trivial.
         apply sepcon_derives. 
          eapply derives_trans; try apply data_at_data_at_.
-               rewrite data_at__memory_block. entailer.
+               rewrite data_at__memory_block. entailer!.
                simpl. rewrite <- Zlength_correct.
                rewrite Zlength_max_zero, HH. cancel.
                reflexivity.
@@ -478,34 +479,37 @@ forward_if PostKeyNull.
      { simpl. rewrite Zlength_max_zero, HH. subst l. split; trivial.
           rewrite int_max_unsigned_eq.
           rewrite int_max_signed_eq in KL2. omega. }
+
      simpl. subst v. remember (map Vint (map Int.repr key)) as KCONT.
+
      (*call memset*)
      clear HH.
      forward_call' (Tsh, Vptr ckb (Int.add ckoff (Int.repr (Zlength key))), l64, Int.zero)
        vret.
-     rewrite <- KL1.
-     match goal with |- _ * _ * ?A * _ * _ * _ |-- _ => 
+     { rewrite <- KL1.
+       match goal with |- _ * _ * ?A * _ * _ * _ |-- _ => 
                   pull_left A end.
-     repeat rewrite sepcon_assoc. apply sepcon_derives; [ | cancel].
-     eapply derives_trans; try apply data_at_data_at_.
+       repeat rewrite sepcon_assoc. apply sepcon_derives; [ | cancel].
+       eapply derives_trans; try apply data_at_data_at_.
                rewrite data_at__memory_block. 
-               rewrite sizeof_Tarray. entailer.
-     rewrite Zmax_spec.
-     rewrite if_false by omega; auto.
-     reflexivity.
-     subst l64.
-     rewrite  sizeof_Tarray.
-     change Int.modulus with (Int.max_unsigned+1).
-     repable_signed. 
-     apply Z.max_r. omega.
-     split; auto. repable_signed.
+               rewrite sizeof_Tarray. entailer!.
+       rewrite Zmax_spec.
+       rewrite if_false by omega; auto.
+       reflexivity.
+       subst l64.
+       rewrite  sizeof_Tarray.
+       change Int.modulus with (Int.max_unsigned+1).
+       repable_signed. 
+       apply Z.max_r. omega.
+     } 
+     { split; auto. repable_signed. }
 
      subst PostIf_j_Len.
-   entailer!.
-   cancel. unfold tarray.
+     entailer!.
+     cancel. unfold tarray.
 
-   destruct (zlt 64 (Zlength key)). omega. rewrite Zlength_correct in g. apply (Nat2Z.inj_ge 64) in g.
-   clear H0 TC0 h1.
+     destruct (zlt 64 (Zlength key)). omega. rewrite Zlength_correct in g. apply (Nat2Z.inj_ge 64) in g.
+     clear H0 TC0 h1.
      remember (64 - Zlength key) as ZK64.
      rewrite (data_at_Tarray_split3a Tsh tuchar 64 noattr (Zlength key)). 2: omega.
               simpl. unfold nat_of_Z. rewrite Zlength_correct, Nat2Z.id.
@@ -515,37 +519,38 @@ forward_if PostKeyNull.
       2: rewrite Zlength_correct, app_length, force_lengthn_length_n, Nat2Z.inj_add; omega.
       2: rewrite Zlength_correct in ge_64_l; omega.
       assert (STO: sizeof tuchar = 1) by reflexivity. rewrite STO, Z.mul_1_l. rewrite Z.mul_1_l.
-      entailer. 
+      entailer!. 
 
      remember (64 - Zlength key) as ZK64. 
       specialize (split_offset_array_at (Z.to_nat ZK64) Tsh tuchar ZK64). intros X. unfold tarray in X. 
-        rewrite X. clear X. entailer.
+        rewrite X. clear X. entailer!.
      remember (64 - Zlength key) as ZK64. 
      assert (F64: false = (Zlength key >? 64)). 
-       rewrite Z.gtb_ltb. symmetry. apply Fcore_Zaux.Zlt_bool_false. omega.
-      rewrite firstn_app1. 2: rewrite force_lengthn_length_n; trivial.
-      rewrite firstn_precise. 2: rewrite length_list_repeat; trivial.
-      rewrite firstn_precise. 2: rewrite force_lengthn_length_n; trivial.
-      assert (NULL: ZK64 - Z.of_nat (Z.to_nat ZK64) = 0).
-        rewrite Z2Nat.id. omega. omega.
-      rewrite NULL.
-      rewrite skipn_short. 2: rewrite length_list_repeat; omega.
-      apply derives_trans
+     { rewrite Z.gtb_ltb. symmetry. apply Fcore_Zaux.Zlt_bool_false. omega. }
+     rewrite firstn_app1. 2: rewrite force_lengthn_length_n; trivial.
+     rewrite firstn_precise. 2: rewrite length_list_repeat; trivial.
+     rewrite firstn_precise. 2: rewrite force_lengthn_length_n; trivial.
+     assert (NULL: ZK64 - Z.of_nat (Z.to_nat ZK64) = 0).
+     { rewrite Z2Nat.id. omega. omega. }
+     rewrite NULL.
+     rewrite skipn_short. 2: rewrite length_list_repeat; omega.
+     apply derives_trans
        with (Q:=data_at Tsh (Tarray tuchar (Z.of_nat (length key)) noattr)
                   (map Vint (map Int.repr key)) (Vptr ckb ckoff) *
                 data_at Tsh (Tarray tuchar (Z.of_nat (Z.to_nat ZK64)) noattr)
                   (list_repeat (Z.to_nat ZK64) (Vint Int.zero))
                   (Vptr ckb (Int.add ckoff (Int.repr (Z.of_nat (length key)))))).
-          cancel.
-          eapply derives_trans; try apply data_at_data_at_.
-          rewrite data_at__memory_block. simpl. entailer.
-          reflexivity. simpl. specialize Int.modulus_pos. omega.
-      apply sepcon_derives.
-      { apply data_at_Tarray_ext_derives. intros i I.
-        apply data_at_triv. unfold Znth. if_tac. trivial. clear H.
-        rewrite nth_force_lengthn.
-        Focus 2. split. omega. destruct I as [Ipos I]. apply Z2Nat.inj_lt in I; trivial.
-                 rewrite Nat2Z.id in I. trivial. omega.
+     { cancel.
+       eapply derives_trans; try apply data_at_data_at_.
+       rewrite data_at__memory_block. simpl. entailer!.
+       reflexivity. simpl. specialize Int.modulus_pos. omega.
+     }
+     { apply sepcon_derives.
+       { apply data_at_Tarray_ext_derives. intros i I.
+         apply data_at_triv. unfold Znth. if_tac. trivial. clear H.
+         rewrite nth_force_lengthn.
+         Focus 2. split. omega. destruct I as [Ipos I]. apply Z2Nat.inj_lt in I; trivial.
+                  rewrite Nat2Z.id in I. trivial. omega.
          assert (Z32: (Z.to_nat i < length key)%nat).
                   clear - I; destruct I as [XX YY]. rewrite Z2Nat.inj_lt in YY.
                   rewrite Nat2Z.id in YY; trivial. trivial. omega. 
@@ -561,25 +566,25 @@ forward_if PostKeyNull.
          rewrite nth_map' with (d':=Z0); trivial. f_equal. f_equal.         
          eapply mkKey_left; trivial. rewrite Zlength_correct. trivial.
          rewrite map_length; trivial. rewrite map_length; trivial.
-      }
-      { unfold offset_val. rewrite skipn_force_lengthn_app. rewrite Z2Nat.id.  
-        rewrite HeqZK64, Zlength_correct.
-        apply data_at_Tarray_ext_derives. rewrite <- Zlength_correct, <- HeqZK64.
-        intros i I.
-        apply data_at_triv. unfold Znth. if_tac. trivial. clear H.
-        rewrite Zlength_correct.
-        destruct (zlt (Z.of_nat (length key)) 0).
-        rewrite <- Zlength_correct in l. omega.
-        rewrite nth_indep with (d:=(default_val tuchar))(d':=Vint (Int.repr 0)).
-        Focus 2.  rewrite length_list_repeat. apply Z2Nat.inj_lt. omega. omega. omega.
-        rewrite nth_list_repeat. rewrite HeqZK64, Zlength_correct in I.
-        remember (Z.to_nat i) as K; destruct K; simpl.
+       }
+       { unfold offset_val. rewrite skipn_force_lengthn_app. rewrite Z2Nat.id.  
+         rewrite HeqZK64, Zlength_correct.
+         apply data_at_Tarray_ext_derives. rewrite <- Zlength_correct, <- HeqZK64.
+         intros i I.
+         apply data_at_triv. unfold Znth. if_tac. trivial. clear H.
+         rewrite Zlength_correct.
+         destruct (zlt (Z.of_nat (length key)) 0).
+         rewrite <- Zlength_correct in l. omega.
+         rewrite nth_indep with (d:=(default_val tuchar))(d':=Vint (Int.repr 0)).
+         Focus 2.  rewrite length_list_repeat. apply Z2Nat.inj_lt. omega. omega. omega.
+         rewrite nth_list_repeat. rewrite HeqZK64, Zlength_correct in I.
+         remember (Z.to_nat i) as K; destruct K; simpl.
          rewrite nth_map' with (d':=Int.zero).
          rewrite nth_map' with (d':=Z0); trivial. f_equal. f_equal.    
          rewrite mkKey_right; trivial. rewrite Zlength_correct. omega.
          rewrite mkKey_length, Nat2Z.id. unfold SHA256.BlockSize. omega.
          rewrite map_length, mkKey_length, Nat2Z.id. unfold SHA256.BlockSize. omega.
-        rewrite nth_skipn. 
+         rewrite nth_skipn. 
          assert (K + Z.to_nat (Z.of_nat (length key) + 1) = Z.to_nat (Z.of_nat (length key) + i))%nat.
             rewrite Z2Nat.inj_add. rewrite Z2Nat.inj_add. rewrite <- HeqK.
             remember (Z.to_nat (Z.of_nat (length key))) as u. simpl. rewrite <- plus_n_Sm. rewrite <- (plus_Snm_nSm u). omega.
@@ -594,53 +599,44 @@ forward_if PostKeyNull.
          rewrite mkKey_length. unfold SHA256.BlockSize. apply (Z2Nat.inj_lt _ 64). omega. omega. omega. 
          rewrite map_length. rewrite mkKey_length. unfold SHA256.BlockSize. apply (Z2Nat.inj_lt _ 64). omega. omega. omega. 
          omega.
-      }
-      reflexivity. rewrite Zlength_correct, length_list_repeat. omega.
-      rewrite Z2Nat.id; omega.
-  }
+       }
+     } 
+     { reflexivity. }
+     { rewrite Zlength_correct, length_list_repeat. omega. }
+     { rewrite Z2Nat.id; omega. }
+   }
 
-  intros. 
-   entailer. unfold POSTCONDITION, abbreviate; simpl. entailer.
+   intros. 
+   entailer!. unfold POSTCONDITION, abbreviate; simpl. entailer!.
    unfold overridePost, initPostKeyNullConditional. 
    if_tac; trivial.
-   entailer.
+   entailer!.
      apply (exp_right cb). apply andp_right. entailer!.
    entailer!.
-     apply (exp_right cofs). normalize. 
-(*     rewrite data_at__isptr. normalize.
-     apply isptrD in H4. destruct H4 as [pb [pofs PAD]].*)
-(*     apply (exp_right Vptr pb pofs).
-   entailer. *)
-     apply (exp_right 1). entailer. 
-(*     apply isptrD in H5. destruct H5 as [ckb [ckoff CK]].
-     apply exp_right with (x:=Vptr ckb ckoff).
-     entailer. cancel.*)
-     if_tac; try omega. cancel.
+     apply (exp_right cofs). normalize. clear H. 
+     apply (exp_right 1). entailer!. 
   }
   { (*key == NULL*)
      forward. normalize. rewrite HeqPostKeyNull. clear  HeqPostKeyNull. normalize.
-     entailer.
+     entailer!.
      unfold initPre, initPostKeyNullConditional.
      destruct key'; try contradiction; simpl in *; subst; simpl in *.
      (*integer*)
         unfold hmacstate_PreInitNull. normalize. rewrite data_at_isptr.
         normalize. apply isptrD in Pctx'. destruct Pctx' as [cb [cofs CTX']].
         subst; simpl in *. 
- (*       apply isptrD in H1. destruct H1 as [pb [pofs PAD]].*)
         apply exp_right with (x:=cb).
         apply exp_right with (x:=cofs).
-        apply exp_right with (x:=0). entailer. (* rewrite PAD. cancel.
-        apply isptrD in H2. destruct H2 as [ckb [ckoff CK]].
-        apply exp_right with (x:=Vptr ckb ckoff). entailer. cancel. *)
+        apply exp_right with (x:=0). entailer!.
         if_tac; try omega. cancel.
           apply exp_right with (x:=r). cancel. 
-          apply exp_right with (x:=v). entailer.
+          apply exp_right with (x:=v). entailer!.
      inversion H.
   }
   { (*side condition of forward_if key != NULL*)
-    intros. entailer. unfold overridePost, normal_ret_assert; simpl. 
+    intros. entailer!. unfold overridePost, normal_ret_assert; simpl. 
     if_tac. simpl. unfold POSTCONDITION, abbreviate, normal_ret_assert.
-       entailer. trivial.
+       entailer!. trivial.
   }
 Qed.
 
